show value equality is decidable

notations.lean
@@ -79,17 +79,684 @@ instance : has_coe (spec × history × env × exp) stack := ⟨λe, stack.top e.
 -- κ · [H, σ, let y = f [ x ] in e]
 notation st `·` `[` R `,` H `,` env `,` `letapp` y `=`:1 f `[` x `]` `in` e `]` := stack.cons st R H env y f x e
 
--- env lookup as function application
+-- to use values, expressions, terms, specs, histories and environments with recursion,
+-- we need to show that the recursion is decreasing, i.e. its parts are smaller than the whole
 
-@[reducible]
-def env.size: env → ℕ := env.rec (λ_, ℕ) 0 (λ_ _ _ n, n + 1)
-instance : has_sizeof env := ⟨env.size⟩
+lemma sizeof_value_func_R {f x: var} {R S: spec} {e: exp} {H: history} {σ: env}:
+      R.sizeof < (value.func f x R S e H σ).sizeof :=
+  begin
+    unfold value.sizeof,
+    rw[add_assoc],
+    rw[add_assoc],
+    rw[add_assoc],
+    rw[add_assoc],
+    rw[add_comm],
+    rw[add_assoc],
+    apply lt_add_of_pos_right,
+    apply lt_add_of_le_of_pos nonneg_of_nat,
+    rw[add_comm],
+    apply lt_add_of_le_of_pos nonneg_of_nat,
+    rw[add_comm],
+    apply lt_add_of_le_of_pos nonneg_of_nat,
+    from zero_lt_one
+  end
+
+lemma sizeof_value_func_S {f x: var} {R S: spec} {e: exp} {H: history} {σ: env}:
+      S.sizeof < (value.func f x R S e H σ).sizeof :=
+  begin
+    unfold value.sizeof,
+    rw[add_assoc],
+    rw[add_assoc],
+    rw[add_assoc],
+    rw[add_comm],
+    rw[add_assoc],
+    apply lt_add_of_pos_right,
+    apply lt_add_of_le_of_pos nonneg_of_nat,
+    rw[add_comm],
+    apply lt_add_of_le_of_pos nonneg_of_nat,
+    rw[add_comm],
+    apply lt_add_of_le_of_pos nonneg_of_nat,
+    rw[add_comm],
+    apply lt_add_of_le_of_pos nonneg_of_nat,
+    from zero_lt_one
+  end
+
+lemma sizeof_value_func_e {f x: var} {R S: spec} {e: exp} {H: history} {σ: env}:
+      e.sizeof < (value.func f x R S e H σ).sizeof :=
+  begin
+    unfold value.sizeof,
+    rw[add_assoc],
+    rw[add_assoc],
+    rw[add_comm],
+    rw[add_assoc],
+    apply lt_add_of_pos_right,
+    apply lt_add_of_le_of_pos nonneg_of_nat,
+    rw[add_comm],
+    apply lt_add_of_le_of_pos nonneg_of_nat,
+    rw[add_comm],
+    apply lt_add_of_le_of_pos nonneg_of_nat,
+    rw[add_comm],
+    apply lt_add_of_le_of_pos nonneg_of_nat,
+    rw[add_comm],
+    apply lt_add_of_le_of_pos nonneg_of_nat,
+    from zero_lt_one
+  end
+
+lemma sizeof_value_func_H {f x: var} {R S: spec} {e: exp} {H: history} {σ: env}:
+      H.sizeof < (value.func f x R S e H σ).sizeof :=
+  begin
+    unfold value.sizeof,
+    rw[add_assoc],
+    rw[add_comm],
+    rw[add_assoc],
+    apply lt_add_of_pos_right,
+    apply lt_add_of_le_of_pos nonneg_of_nat,
+    rw[add_comm],
+    apply lt_add_of_le_of_pos nonneg_of_nat,
+    rw[add_comm],
+    apply lt_add_of_le_of_pos nonneg_of_nat,
+    rw[add_comm],
+    apply lt_add_of_le_of_pos nonneg_of_nat,
+    rw[add_comm],
+    apply lt_add_of_le_of_pos nonneg_of_nat,
+    rw[add_comm],
+    apply lt_add_of_le_of_pos nonneg_of_nat,
+    from zero_lt_one
+  end
+
+lemma sizeof_value_func_σ {f x: var} {R S: spec} {e: exp} {H: history} {σ: env}:
+      σ.sizeof < (value.func f x R S e H σ).sizeof :=
+  begin
+    unfold value.sizeof,
+    rw[add_comm],
+    rw[add_assoc],
+    apply lt_add_of_pos_right,
+    rw[add_comm],
+    apply lt_add_of_le_of_pos nonneg_of_nat,
+    rw[add_comm],
+    apply lt_add_of_le_of_pos nonneg_of_nat,
+    rw[add_comm],
+    apply lt_add_of_le_of_pos nonneg_of_nat,
+    rw[add_comm],
+    apply lt_add_of_le_of_pos nonneg_of_nat,
+    rw[add_comm],
+    apply lt_add_of_le_of_pos nonneg_of_nat,
+    from zero_lt_one
+  end
+
+lemma sizeof_exp_true {x: var} {e: exp}:
+      e.sizeof < (exp.true x e).sizeof :=
+  begin
+    unfold exp.sizeof,
+    rw[add_comm],
+    apply lt_add_of_pos_right,
+    rw[add_comm],
+    apply lt_add_of_le_of_pos nonneg_of_nat,
+    from zero_lt_one
+  end
+
+lemma sizeof_exp_false {x: var} {e: exp}:
+      e.sizeof < (exp.false x e).sizeof :=
+  begin
+    unfold exp.sizeof,
+    rw[add_comm],
+    apply lt_add_of_pos_right,
+    rw[add_comm],
+    apply lt_add_of_le_of_pos nonneg_of_nat,
+    from zero_lt_one
+  end
+
+lemma sizeof_exp_num {x: var} {n: ℤ} {e: exp}:
+      e.sizeof < (exp.num x n e).sizeof :=
+  begin
+    unfold exp.sizeof,
+    rw[add_comm],
+    apply lt_add_of_pos_right,
+    rw[add_comm],
+    apply lt_add_of_le_of_pos nonneg_of_nat,
+    rw[add_comm],
+    apply lt_add_of_le_of_pos nonneg_of_nat,
+    from zero_lt_one
+  end
+
+lemma sizeof_exp_func_R {f x: var} {R S: spec} {e₁ e₂: exp}:
+      R.sizeof < (exp.func f x R S e₁ e₂).sizeof :=
+  begin
+    unfold exp.sizeof,
+    rw[add_assoc],
+    rw[add_assoc],
+    rw[add_assoc],
+    rw[add_comm],
+    rw[add_assoc],
+    apply lt_add_of_pos_right,
+    apply lt_add_of_le_of_pos nonneg_of_nat,
+    rw[add_comm],
+    apply lt_add_of_le_of_pos nonneg_of_nat,
+    rw[add_comm],
+    apply lt_add_of_le_of_pos nonneg_of_nat,
+    from zero_lt_one
+  end
+
+lemma sizeof_exp_func_S {f x: var} {R S: spec} {e₁ e₂: exp}:
+      S.sizeof < (exp.func f x R S e₁ e₂).sizeof :=
+  begin
+    unfold exp.sizeof,
+    rw[add_assoc],
+    rw[add_assoc],
+    rw[add_comm],
+    rw[add_assoc],
+    apply lt_add_of_pos_right,
+    apply lt_add_of_le_of_pos nonneg_of_nat,
+    rw[add_comm],
+    apply lt_add_of_le_of_pos nonneg_of_nat,
+    rw[add_comm],
+    apply lt_add_of_le_of_pos nonneg_of_nat,
+    rw[add_comm],
+    apply lt_add_of_le_of_pos nonneg_of_nat,
+    from zero_lt_one
+  end
+
+lemma sizeof_exp_func_e₁ {f x: var} {R S: spec} {e₁ e₂: exp}:
+      e₁.sizeof < (exp.func f x R S e₁ e₂).sizeof :=
+  begin
+    unfold exp.sizeof,
+    rw[add_assoc],
+    rw[add_comm],
+    rw[add_assoc],
+    apply lt_add_of_pos_right,
+    apply lt_add_of_le_of_pos nonneg_of_nat,
+    rw[add_comm],
+    apply lt_add_of_le_of_pos nonneg_of_nat,
+    rw[add_comm],
+    apply lt_add_of_le_of_pos nonneg_of_nat,
+    rw[add_comm],
+    apply lt_add_of_le_of_pos nonneg_of_nat,
+    rw[add_comm],
+    apply lt_add_of_le_of_pos nonneg_of_nat,
+    from zero_lt_one
+  end
+
+lemma sizeof_exp_func_e₂ {f x: var} {R S: spec} {e₁ e₂: exp}:
+      e₂.sizeof < (exp.func f x R S e₁ e₂).sizeof :=
+  begin
+    unfold exp.sizeof,
+    rw[add_comm],
+    rw[add_assoc],
+    apply lt_add_of_pos_right,
+    rw[add_comm],
+    apply lt_add_of_le_of_pos nonneg_of_nat,
+    rw[add_comm],
+    apply lt_add_of_le_of_pos nonneg_of_nat,
+    rw[add_comm],
+    apply lt_add_of_le_of_pos nonneg_of_nat,
+    rw[add_comm],
+    apply lt_add_of_le_of_pos nonneg_of_nat,
+    from zero_lt_one
+  end
+
+lemma sizeof_exp_unop {x y: var} {op: unop} {e: exp}:
+      e.sizeof < (exp.unop y op x e).sizeof :=
+  begin
+    unfold exp.sizeof,
+    rw[add_comm],
+    apply lt_add_of_pos_right,
+    rw[add_comm],
+    apply lt_add_of_le_of_pos nonneg_of_nat,
+    rw[add_comm],
+    apply lt_add_of_le_of_pos nonneg_of_nat,
+    rw[add_comm],
+    apply lt_add_of_le_of_pos nonneg_of_nat,
+    from zero_lt_one
+  end
+
+lemma sizeof_exp_binop {x y z: var} {op: binop} {e: exp}:
+      e.sizeof < (exp.binop z op x y e).sizeof :=
+  begin
+    unfold exp.sizeof,
+    rw[add_comm],
+    apply lt_add_of_pos_right,
+    rw[add_comm],
+    apply lt_add_of_le_of_pos nonneg_of_nat,
+    rw[add_comm],
+    apply lt_add_of_le_of_pos nonneg_of_nat,
+    rw[add_comm],
+    apply lt_add_of_le_of_pos nonneg_of_nat,
+    rw[add_comm],
+    apply lt_add_of_le_of_pos nonneg_of_nat,
+    from zero_lt_one
+  end
+
+lemma sizeof_exp_app {x y z: var} {e: exp}:
+      e.sizeof < (exp.app z x y e).sizeof :=
+  begin
+    unfold exp.sizeof,
+    rw[add_comm],
+    apply lt_add_of_pos_right,
+    rw[add_comm],
+    apply lt_add_of_le_of_pos nonneg_of_nat,
+    rw[add_comm],
+    apply lt_add_of_le_of_pos nonneg_of_nat,
+    rw[add_comm],
+    apply lt_add_of_le_of_pos nonneg_of_nat,
+    from zero_lt_one
+  end
+
+lemma sizeof_exp_ite_e₁ {x: var} {e₁ e₂: exp}:
+      e₁.sizeof < (exp.ite x e₁ e₂).sizeof :=
+  begin
+    unfold exp.sizeof,
+    rw[add_assoc],
+    rw[add_comm],
+    rw[add_assoc],
+    apply lt_add_of_pos_right,
+    apply lt_add_of_le_of_pos nonneg_of_nat,
+    rw[add_comm],
+    apply lt_add_of_le_of_pos nonneg_of_nat,
+    from zero_lt_one
+  end
+
+lemma sizeof_exp_ite_e₂ {x: var} {e₁ e₂: exp}:
+      e₂.sizeof < (exp.ite x e₁ e₂).sizeof :=
+  begin
+    unfold exp.sizeof,
+    rw[add_comm],
+    rw[add_assoc],
+    apply lt_add_of_pos_right,
+    rw[add_comm],
+    apply lt_add_of_le_of_pos nonneg_of_nat,
+    from zero_lt_one
+  end
+
+lemma sizeof_term_value {v: value}:
+      v.sizeof < (term.value v).sizeof :=
+  begin
+    unfold term.sizeof,
+    rw[add_comm],
+    apply lt_add_of_pos_right,
+    from zero_lt_one
+  end
+
+lemma sizeof_term_unop {op: unop} {t: term}:
+      t.sizeof < (term.unop op t).sizeof :=
+  begin
+    unfold term.sizeof,
+    rw[add_comm],
+    apply lt_add_of_pos_right,
+    rw[add_comm],
+    apply lt_add_of_le_of_pos nonneg_of_nat,
+    from zero_lt_one
+  end
+
+lemma sizeof_term_binop₁ {op: binop} {t₁ t₂: term}:
+      t₁.sizeof < (term.binop op t₁ t₂).sizeof :=
+  begin
+    unfold term.sizeof,
+    rw[add_assoc],
+    rw[add_comm],
+    rw[add_assoc],
+    apply lt_add_of_pos_right,
+    apply lt_add_of_le_of_pos nonneg_of_nat,
+    rw[add_comm],
+    apply lt_add_of_le_of_pos nonneg_of_nat,
+    from zero_lt_one
+  end
+
+lemma sizeof_term_binop₂ {op: binop} {t₁ t₂: term}:
+      t₂.sizeof < (term.binop op t₁ t₂).sizeof :=
+  begin
+    unfold term.sizeof,
+    rw[add_assoc],
+    rw[add_comm],
+    rw[add_assoc],
+    rw[add_comm],
+    rw[add_assoc],
+    apply lt_add_of_pos_right,
+    rw[add_comm],
+    apply lt_add_of_le_of_pos nonneg_of_nat,
+    rw[add_comm],
+    apply lt_add_of_le_of_pos nonneg_of_nat,
+    from zero_lt_one
+  end
+
+lemma sizeof_term_app₁ {t₁ t₂: term}:
+      t₁.sizeof < (term.app t₁ t₂).sizeof :=
+  begin
+    unfold term.sizeof,
+    rw[add_assoc],
+    rw[add_comm],
+    rw[add_assoc],
+    apply lt_add_of_pos_right,
+    apply lt_add_of_le_of_pos nonneg_of_nat,
+    from zero_lt_one
+  end
+
+lemma sizeof_term_app₂ {t₁ t₂: term}:
+      t₂.sizeof < (term.app t₁ t₂).sizeof :=
+  begin
+    unfold term.sizeof,
+    rw[add_assoc],
+    rw[add_comm],
+    rw[add_assoc],
+    rw[add_comm],
+    rw[add_assoc],
+    apply lt_add_of_pos_right,
+    rw[add_comm],
+    apply lt_add_of_le_of_pos nonneg_of_nat,
+    from zero_lt_one
+  end
+
+lemma sizeof_spec_term {t: term}:
+      t.sizeof < (spec.term t).sizeof :=
+  begin
+    unfold spec.sizeof,
+    rw[add_comm],
+    apply lt_add_of_pos_right,
+    from zero_lt_one
+  end
+
+lemma sizeof_spec_not {R: spec}:
+      R.sizeof < R.not.sizeof :=
+  begin
+    unfold spec.sizeof,
+    rw[add_comm],
+    apply lt_add_of_pos_right,
+    from zero_lt_one
+  end
+
+lemma sizeof_spec_and₁ {R S: spec}:
+      R.sizeof < (spec.and R S).sizeof :=
+  begin
+    unfold spec.sizeof,
+    rw[add_assoc],
+    rw[add_comm],
+    rw[add_assoc],
+    apply lt_add_of_pos_right,
+    change 0 < sizeof S + 1,
+    apply lt_add_of_le_of_pos nonneg_of_nat,
+    from zero_lt_one
+  end
+
+lemma sizeof_spec_and₂ {R S: spec}:
+      S.sizeof < (spec.and R S).sizeof :=
+  begin
+    unfold spec.sizeof,
+    rw[add_comm],
+    apply lt_add_of_pos_right,
+    change 0 < 1 + sizeof R,
+    rw[add_comm],
+    apply lt_add_of_le_of_pos nonneg_of_nat,
+    from zero_lt_one
+  end
+
+lemma sizeof_spec_or₁ {R S: spec}:
+      R.sizeof < (spec.or R S).sizeof :=
+  begin
+    unfold spec.sizeof,
+    rw[add_assoc],
+    rw[add_comm],
+    rw[add_assoc],
+    apply lt_add_of_pos_right,
+    change 0 < sizeof S + 1,
+    apply lt_add_of_le_of_pos nonneg_of_nat,
+    from zero_lt_one
+  end
+
+lemma sizeof_spec_or₂ {R S: spec}:
+      S.sizeof < (spec.or R S).sizeof :=
+  begin
+    unfold spec.sizeof,
+    rw[add_comm],
+    apply lt_add_of_pos_right,
+    change 0 < 1 + sizeof R,
+    rw[add_comm],
+    apply lt_add_of_le_of_pos nonneg_of_nat,
+    from zero_lt_one
+  end
+
+lemma sizeof_spec_func_t {f: term} {x: var} {R S: spec}:
+      f.sizeof < (spec.func f x R S).sizeof :=
+  begin
+    unfold spec.sizeof,
+    rw[add_assoc],
+    rw[add_assoc],
+    rw[add_assoc],
+    rw[add_comm],
+    rw[add_assoc],
+    apply lt_add_of_pos_right,
+    apply lt_add_of_le_of_pos nonneg_of_nat,
+    from zero_lt_one
+  end
+
+lemma sizeof_spec_func_R {f: term} {x: var} {R S: spec}:
+      R.sizeof < (spec.func f x R S).sizeof :=
+  begin
+    unfold spec.sizeof,
+    rw[add_assoc],
+    rw[add_comm],
+    rw[add_assoc],
+    apply lt_add_of_pos_right,
+    change 0 < sizeof S + (1 + sizeof f + sizeof x),
+    apply lt_add_of_le_of_pos nonneg_of_nat,
+    rw[add_comm],
+    apply lt_add_of_le_of_pos nonneg_of_nat,
+    rw[add_comm],
+    apply lt_add_of_le_of_pos nonneg_of_nat,
+    from zero_lt_one
+  end
+
+lemma sizeof_spec_func_S {f: term} {x: var} {R S: spec}:
+      S.sizeof < (spec.func f x R S).sizeof :=
+  begin
+    unfold spec.sizeof,
+    rw[add_comm],
+    apply lt_add_of_pos_right,
+    change 0 < 1 + sizeof f + sizeof x + sizeof R,
+    rw[add_comm],
+    apply lt_add_of_le_of_pos nonneg_of_nat,
+    rw[add_comm],
+    apply lt_add_of_le_of_pos nonneg_of_nat,
+    rw[add_comm],
+    apply lt_add_of_le_of_pos nonneg_of_nat,
+    from zero_lt_one
+  end
+
+lemma sizeof_env_rest {σ: env} {x: var} {v: value}:
+      σ.sizeof < (σ[x↦v]).sizeof :=
+  begin
+    unfold env.sizeof,
+    rw[add_assoc],
+    rw[add_assoc],
+    rw[add_comm],
+    rw[add_assoc],
+    apply lt_add_of_pos_right,
+    change 0 < sizeof x + (sizeof v + 1),
+    apply lt_add_of_le_of_pos nonneg_of_nat,
+    apply lt_add_of_le_of_pos nonneg_of_nat,
+    from zero_lt_one
+  end
+
+lemma sizeof_env_value {σ: env} {x: var} {v: value}:
+      v.sizeof < (σ[x↦v]).sizeof :=
+  begin
+    unfold env.sizeof,
+    rw[add_comm],
+    apply lt_add_of_pos_right,
+    rw[add_comm],
+    apply lt_add_of_le_of_pos nonneg_of_nat,
+    rw[add_comm],
+    apply lt_add_of_le_of_pos nonneg_of_nat,
+    from zero_lt_one
+  end
+
+lemma sizeof_history_rest {f x: var} {R S: spec} {e: exp} {H₁ H₂: history} {σ: env} {v: value}:
+      H₁.sizeof < (history.call H₁ f x R S e H₂ σ v).sizeof :=
+  begin
+    unfold history.sizeof,
+    rw[add_assoc],
+    rw[add_assoc],
+    rw[add_assoc],
+    rw[add_assoc],
+    rw[add_assoc],
+    rw[add_assoc],
+    rw[add_assoc],
+    rw[add_assoc],
+    rw[add_comm],
+    rw[add_assoc],
+    apply lt_add_of_pos_right,
+    apply lt_add_of_le_of_pos nonneg_of_nat,
+    from zero_lt_one
+  end
+
+lemma sizeof_history_R {f x: var} {R S: spec} {e: exp} {H₁ H₂: history} {σ: env} {v: value}:
+      R.sizeof < (history.call H₁ f x R S e H₂ σ v).sizeof :=
+  begin
+    unfold history.sizeof,
+    rw[add_assoc],
+    rw[add_assoc],
+    rw[add_assoc],
+    rw[add_assoc],
+    rw[add_assoc],
+    rw[add_comm],
+    rw[add_assoc],
+    apply lt_add_of_pos_right,
+    apply lt_add_of_le_of_pos nonneg_of_nat,
+    rw[add_comm],
+    apply lt_add_of_le_of_pos nonneg_of_nat,
+    rw[add_comm],
+    apply lt_add_of_le_of_pos nonneg_of_nat,
+    rw[add_comm],
+    apply lt_add_of_le_of_pos nonneg_of_nat,
+    from zero_lt_one
+  end
+
+lemma sizeof_history_S {f x: var} {R S: spec} {e: exp} {H₁ H₂: history} {σ: env} {v: value}:
+      S.sizeof < (history.call H₁ f x R S e H₂ σ v).sizeof :=
+  begin
+    unfold history.sizeof,
+    rw[add_assoc],
+    rw[add_assoc],
+    rw[add_assoc],
+    rw[add_assoc],
+    rw[add_comm],
+    rw[add_assoc],
+    apply lt_add_of_pos_right,
+    apply lt_add_of_le_of_pos nonneg_of_nat,
+    rw[add_comm],
+    apply lt_add_of_le_of_pos nonneg_of_nat,
+    rw[add_comm],
+    apply lt_add_of_le_of_pos nonneg_of_nat,
+    rw[add_comm],
+    apply lt_add_of_le_of_pos nonneg_of_nat,
+    rw[add_comm],
+    apply lt_add_of_le_of_pos nonneg_of_nat,
+    from zero_lt_one
+  end
+
+lemma sizeof_history_e {f x: var} {R S: spec} {e: exp} {H₁ H₂: history} {σ: env} {v: value}:
+      e.sizeof < (history.call H₁ f x R S e H₂ σ v).sizeof :=
+  begin
+    unfold history.sizeof,
+    rw[add_assoc],
+    rw[add_assoc],
+    rw[add_assoc],
+    rw[add_comm],
+    rw[add_assoc],
+    apply lt_add_of_pos_right,
+    apply lt_add_of_le_of_pos nonneg_of_nat,
+    rw[add_comm],
+    apply lt_add_of_le_of_pos nonneg_of_nat,
+    rw[add_comm],
+    apply lt_add_of_le_of_pos nonneg_of_nat,
+    rw[add_comm],
+    apply lt_add_of_le_of_pos nonneg_of_nat,
+    rw[add_comm],
+    apply lt_add_of_le_of_pos nonneg_of_nat,
+    rw[add_comm],
+    apply lt_add_of_le_of_pos nonneg_of_nat,
+    from zero_lt_one
+  end
+
+lemma sizeof_history_H {f x: var} {R S: spec} {e: exp} {H₁ H₂: history} {σ: env} {v: value}:
+      H₂.sizeof < (history.call H₁ f x R S e H₂ σ v).sizeof :=
+  begin
+    unfold history.sizeof,
+    rw[add_assoc],
+    rw[add_assoc],
+    rw[add_comm],
+    rw[add_assoc],
+    apply lt_add_of_pos_right,
+    apply lt_add_of_le_of_pos nonneg_of_nat,
+    rw[add_comm],
+    apply lt_add_of_le_of_pos nonneg_of_nat,
+    rw[add_comm],
+    apply lt_add_of_le_of_pos nonneg_of_nat,
+    rw[add_comm],
+    apply lt_add_of_le_of_pos nonneg_of_nat,
+    rw[add_comm],
+    apply lt_add_of_le_of_pos nonneg_of_nat,
+    rw[add_comm],
+    apply lt_add_of_le_of_pos nonneg_of_nat,
+    rw[add_comm],
+    apply lt_add_of_le_of_pos nonneg_of_nat,
+    from zero_lt_one
+  end
+
+lemma sizeof_history_σ {f x: var} {R S: spec} {e: exp} {H₁ H₂: history} {σ: env} {v: value}:
+      σ.sizeof < (history.call H₁ f x R S e H₂ σ v).sizeof :=
+  begin
+    unfold history.sizeof,
+    rw[add_assoc],
+    rw[add_comm],
+    rw[add_assoc],
+    apply lt_add_of_pos_right,
+    apply lt_add_of_le_of_pos nonneg_of_nat,
+    rw[add_comm],
+    apply lt_add_of_le_of_pos nonneg_of_nat,
+    rw[add_comm],
+    apply lt_add_of_le_of_pos nonneg_of_nat,
+    rw[add_comm],
+    apply lt_add_of_le_of_pos nonneg_of_nat,
+    rw[add_comm],
+    apply lt_add_of_le_of_pos nonneg_of_nat,
+    rw[add_comm],
+    apply lt_add_of_le_of_pos nonneg_of_nat,
+    rw[add_comm],
+    apply lt_add_of_le_of_pos nonneg_of_nat,
+    rw[add_comm],
+    apply lt_add_of_le_of_pos nonneg_of_nat,
+    from zero_lt_one
+  end
+
+lemma sizeof_history_v {f x: var} {R S: spec} {e: exp} {H₁ H₂: history} {σ: env} {v: value}:
+      v.sizeof < (history.call H₁ f x R S e H₂ σ v).sizeof :=
+  begin
+    unfold history.sizeof,
+    rw[add_comm],
+    rw[add_assoc],
+    rw[add_assoc],
+    rw[add_assoc],
+    rw[add_assoc],
+    rw[add_assoc],
+    rw[add_assoc],
+    rw[add_assoc],
+    apply lt_add_of_pos_right,
+    rw[add_comm],
+    apply lt_add_of_le_of_pos nonneg_of_nat,
+    from zero_lt_one
+  end
+
+-- env lookup as function application
 
 def env.apply: env → var → option value
 | env.empty _ := none
 | (σ[x↦v]) y :=
-  have σ.size < (σ[x ↦ v].size), from lt_of_add_one,
+  have σ.sizeof < (σ[x↦v]).sizeof, from sizeof_env_rest,
   if x = y ∧ option.is_none (σ.apply y) then v else σ.apply y
+
+using_well_founded {
+  rel_tac := λ _ _, `[exact ⟨_, measure_wf (λ e, e.1.sizeof)⟩],
+  dec_tac := tactic.assumption
+}
 
 def env.rest: env → env
 | env.empty := env.empty
@@ -108,16 +775,6 @@ def env.dom (σ: env): set var := λx, x ∈ σ
 -- spec to prop coercion
 
 @[reducible]
-def spec.size: spec → ℕ := spec.rec (λ_, ℕ)
-  (λ_, 0)
-  (λ_ n, n + 1)
-  (λ_ _ n m , n + m + 1)
-  (λ_ _ n m , n + m + 1)
-  (λ_ _ _ _ n m , n + m + 1)
-
-instance : has_sizeof spec := ⟨spec.size⟩
-
-@[reducible]
 def prop.func (f: term) (x: var) (P: prop) (Q: prop): prop := 
   term.unop unop.isFunc f ⋀
   prop.forallc x f (prop.implies P (prop.pre f x) ⋀
@@ -126,20 +783,25 @@ def prop.func (f: term) (x: var) (P: prop) (Q: prop): prop :=
 def spec.to_prop : spec → prop
 | (spec.term t)       := prop.term t
 | (spec.not S)        :=
-    have S.size < S.not.size, from lt_of_add_one,
+    have S.sizeof < S.not.sizeof, from sizeof_spec_not,
     prop.not S.to_prop
 | (spec.and R S)      :=
-    have R.size < (R ⋀ S).size, from lt_of_add.left,
-    have S.size < (R ⋀ S).size, from lt_of_add.right,
+    have R.sizeof < (R ⋀ S).sizeof, from sizeof_spec_and₁,
+    have S.sizeof < (R ⋀ S).sizeof, from sizeof_spec_and₂,
     R.to_prop ⋀ S.to_prop
 | (spec.or R S)       :=
-    have R.size < (R ⋁ S).size, from lt_of_add.left,
-    have S.size < (R ⋁ S).size, from lt_of_add.right,
+    have R.sizeof < (R ⋁ S).sizeof, from sizeof_spec_or₁,
+    have S.sizeof < (R ⋁ S).sizeof, from sizeof_spec_or₂,
     R.to_prop ⋁ S.to_prop
 | (spec.func f x R S) :=
-    have R.size < (R ⋀ S).size, from lt_of_add.left,
-    have S.size < (R ⋀ S).size, from lt_of_add.right,
+    have R.sizeof < (spec.func f x R S).sizeof, from sizeof_spec_func_R,
+    have S.sizeof < (spec.func f x R S).sizeof, from sizeof_spec_func_S,
     prop.func f x R.to_prop S.to_prop
+
+using_well_founded {
+  rel_tac := λ _ _, `[exact ⟨_, measure_wf (λ e, e.sizeof)⟩],
+  dec_tac := tactic.assumption
+}
 
 instance spec_to_prop : has_coe spec prop := ⟨spec.to_prop⟩
 
@@ -268,3 +930,1172 @@ constant prop.instantiated_p: prop → vc
 
 constant valid : vc → Prop
 notation `⊨` p: 20 := valid p
+
+-- value eq value decidable
+
+instance : decidable_eq unop := by tactic.mk_dec_eq_instance
+instance : decidable_eq binop := by tactic.mk_dec_eq_instance
+
+def wf_measure : has_well_founded
+(psum (Σ' (v₁ : value), value)
+  (psum (Σ' (e₁ : exp), exp)
+    (psum (Σ' (t₁ : term), term)
+      (psum (Σ' (R : spec), spec)
+        (psum (Σ' (σ₁ : env), env)
+          (Σ' (H₁ : history), history))))))
+:= ⟨_, measure_wf $ λ s,
+  match s with
+  | psum.inl a := a.1.sizeof
+  | psum.inr (psum.inl a) := a.1.sizeof
+  | psum.inr (psum.inr (psum.inl a)) := a.1.sizeof
+  | psum.inr (psum.inr (psum.inr (psum.inl a))) := a.1.sizeof
+  | psum.inr (psum.inr (psum.inr (psum.inr (psum.inl a)))) := a.1.sizeof
+  | psum.inr (psum.inr (psum.inr (psum.inr (psum.inr a)))) := a.1.sizeof
+  end⟩
+
+mutual def value.dec_eq, exp.dec_eq, term.dec_eq, spec.dec_eq, env.dec_eq, history.dec_eq
+
+with value.dec_eq : ∀ (v₁ v₂: value), decidable (v₁ = v₂)
+| v₁ v₂ :=
+  let z := v₁ in
+  have h: z = v₁, from rfl,
+  value.cases_on (λv₁, (z = v₁) → decidable (v₁ = v₂)) v₁ (
+    assume : z = value.true,
+    show decidable (value.true = v₂), from
+    value.cases_on (λv₂, decidable (value.true = v₂)) v₂ (
+      show decidable (value.true = value.true), from is_true rfl
+    ) (
+      have value.true ≠ value.false, by contradiction,
+      show decidable (value.true = value.false), from is_false this
+    ) (
+      assume n: ℤ,
+      have value.true ≠ value.num n, by contradiction,
+      show decidable (value.true = value.num n), from is_false this
+    ) (
+      assume f x R S e H σ, 
+      have value.true ≠ value.func f x R S e H σ, by contradiction,
+      show decidable (value.true = value.func f x R S e H σ), from is_false this
+    )
+  )
+  (
+    assume : z = value.false,
+    show decidable (value.false = v₂), from
+    value.cases_on (λv₂, decidable (value.false = v₂)) v₂ (
+      have value.false ≠ value.true, by contradiction,
+      show decidable (value.false = value.true), from is_false this
+    ) (
+      show decidable (value.false = value.false), from is_true rfl
+    ) (
+      assume n: ℤ,
+      have value.false ≠ value.num n, by contradiction,
+      show decidable (value.false = value.num n), from is_false this
+    ) (
+      assume f x R S e H σ, 
+      have value.false ≠ value.func f x R S e H σ, by contradiction,
+      show decidable (value.false = value.func f x R S e H σ), from is_false this
+    )
+   ) (
+    assume n₁: ℤ,
+    assume : z = value.num n₁,
+    show decidable (value.num n₁ = v₂), from
+    value.cases_on (λv₂, decidable (value.num n₁ = v₂)) v₂ (
+      have value.num n₁ ≠ value.true, by contradiction,
+      show decidable (value.num n₁ = value.true), from is_false this
+    ) (
+      have value.num n₁ ≠ value.false, by contradiction,
+      show decidable (value.num n₁ = value.false), from is_false this
+    ) (
+      assume n₂: ℤ,
+      if h: n₁ = n₂ then (
+        have value.num n₁ = value.num n₂, from h ▸ rfl,
+        show decidable (value.num n₁ = value.num n₂), from is_true this
+      ) else (
+        have value.num n₁ ≠ value.num n₂, from (
+          assume : value.num n₁ = value.num n₂,
+          have n₁ = n₂, from value.num.inj this,
+          show «false», from h this
+        ),
+        show decidable (value.num n₁ = value.num n₂), from is_false this
+      )
+    ) (
+      assume f x R S e H σ, 
+      have value.num n₁ ≠ value.func f x R S e H σ, by contradiction,
+      show decidable (value.num n₁ = value.func f x R S e H σ), from is_false this
+    )
+  )
+  (
+    assume f₁ x₁ R₁ S₁ e₁ H₁ σ₁, 
+    assume : z = value.func f₁ x₁ R₁ S₁ e₁ H₁ σ₁,
+    have v₁_is_func: v₁ = value.func f₁ x₁ R₁ S₁ e₁ H₁ σ₁, from eq.trans h this,
+    show decidable (value.func f₁ x₁ R₁ S₁ e₁ H₁ σ₁ = v₂), from
+    value.cases_on (λv₂, decidable (value.func f₁ x₁ R₁ S₁ e₁ H₁ σ₁ = v₂)) v₂ (
+      have value.func f₁ x₁ R₁ S₁ e₁ H₁ σ₁ ≠ value.true, by contradiction,
+      show decidable (value.func f₁ x₁ R₁ S₁ e₁ H₁ σ₁ = value.true), from is_false this
+    ) (
+      have value.func f₁ x₁ R₁ S₁ e₁ H₁ σ₁ ≠ value.false, by contradiction,
+      show decidable (value.func f₁ x₁ R₁ S₁ e₁ H₁ σ₁ = value.false), from is_false this
+    ) (
+      assume n: ℤ,
+      have value.func f₁ x₁ R₁ S₁ e₁ H₁ σ₁ ≠ value.num n, by contradiction,
+      show decidable (value.func f₁ x₁ R₁ S₁ e₁ H₁ σ₁ = value.num n), from is_false this
+    ) (
+      assume f₂ x₂ R₂ S₂ e₂ H₂ σ₂,
+      have R₁.sizeof < v₁.sizeof, from v₁_is_func.symm ▸ sizeof_value_func_R,
+      have decidable (R₁ = R₂), from spec.dec_eq R₁ R₂,
+      have S₁.sizeof < v₁.sizeof, from v₁_is_func.symm ▸ sizeof_value_func_S,
+      have decidable (S₁ = S₂), from spec.dec_eq S₁ S₂,
+      have e₁.sizeof < v₁.sizeof, from v₁_is_func.symm ▸ sizeof_value_func_e,
+      have decidable (e₁ = e₂), from exp.dec_eq e₁ e₂,
+      have H₁.sizeof < v₁.sizeof, from v₁_is_func.symm ▸ sizeof_value_func_H,
+      have decidable (H₁ = H₂), from history.dec_eq H₁ H₂,
+      have σ₁.sizeof < v₁.sizeof, from v₁_is_func.symm ▸ sizeof_value_func_σ,
+      have decidable (σ₁ = σ₂), from env.dec_eq σ₁ σ₂,
+
+      if h: (f₁ = f₂) ∧ (x₁ = x₂) ∧ (R₁ = R₂) ∧ (S₁ = S₂) ∧ (e₁ = e₂) ∧ (H₁ = H₂) ∧ (σ₁ = σ₂) then (
+        have value.func f₁ x₁ R₁ S₁ e₁ H₁ σ₁ = value.func f₂ x₂ R₂ S₂ e₂ H₂ σ₂,
+        from h.left ▸ h.right.left ▸ h.right.right.left ▸ h.right.right.right.left ▸
+             h.right.right.right.right.left ▸ h.right.right.right.right.right.left ▸
+             h.right.right.right.right.right.right ▸ rfl,
+        show decidable (value.func f₁ x₁ R₁ S₁ e₁ H₁ σ₁ = value.func f₂ x₂ R₂ S₂ e₂ H₂ σ₂),
+        from is_true this
+      ) else (
+        have value.func f₁ x₁ R₁ S₁ e₁ H₁ σ₁ ≠ value.func f₂ x₂ R₂ S₂ e₂ H₂ σ₂, from (
+          assume : value.func f₁ x₁ R₁ S₁ e₁ H₁ σ₁ = value.func f₂ x₂ R₂ S₂ e₂ H₂ σ₂,
+          show «false», from h (value.func.inj this)
+        ),
+        show decidable (value.func f₁ x₁ R₁ S₁ e₁ H₁ σ₁ = value.func f₂ x₂ R₂ S₂ e₂ H₂ σ₂),
+        from is_false this
+      )
+    )
+  ) rfl
+
+with exp.dec_eq : ∀ (e₁ e₂: exp), decidable (e₁ = e₂)
+| e₁ e₂ :=
+  let z := e₁ in
+  have h: z = e₁, from rfl,
+  exp.cases_on (λe₁, (z = e₁) → decidable (e₁ = e₂)) e₁ (
+    assume x₁ e₁',
+    assume : z = exp.true x₁ e₁',
+    have e₁_is_tru: e₁ = exp.true x₁ e₁', from eq.trans h this,
+    show decidable (exp.true x₁ e₁' = e₂),
+    from exp.cases_on (λe₂, decidable (exp.true x₁ e₁' = e₂)) e₂ (
+      assume x₂ e₂',
+      have e₁'.sizeof < e₁.sizeof, from e₁_is_tru.symm ▸ sizeof_exp_true,
+      have decidable (e₁' = e₂'), from exp.dec_eq e₁' e₂',
+      if h: (x₁ = x₂) ∧ (e₁' = e₂') then (
+        have exp.true x₁ e₁' = exp.true x₂ e₂',
+        from h.left ▸ h.right ▸ rfl,
+        show decidable (exp.true x₁ e₁' = exp.true x₂ e₂'),
+        from is_true this
+      ) else (
+        have exp.true x₁ e₁' ≠ exp.true x₂ e₂', from (
+          assume : exp.true x₁ e₁' = exp.true x₂ e₂',
+          show «false», from h (exp.true.inj this)
+        ),
+        show decidable (exp.true x₁ e₁' = exp.true x₂ e₂'),
+        from is_false this
+      )
+    ) (
+      assume x₂ e₂',
+      have exp.true x₁ e₁' ≠ exp.false x₂ e₂', by contradiction,
+      show decidable (exp.true x₁ e₁' = exp.false x₂ e₂'), from is_false this
+    ) (
+      assume x₂ n₂ e₂',
+      have exp.true x₁ e₁' ≠ exp.num x₂ n₂ e₂', by contradiction,
+      show decidable (exp.true x₁ e₁' = exp.num x₂ n₂ e₂'), from is_false this
+    ) (
+      assume f₂ x₂ R₂ S₂ e₂' e₂'',
+      have exp.true x₁ e₁' ≠ exp.func f₂ x₂ R₂ S₂ e₂' e₂'', by contradiction,
+      show decidable (exp.true x₁ e₁' = exp.func f₂ x₂ R₂ S₂ e₂' e₂''), from is_false this
+    ) (
+      assume x₂ op₂ y₂ e₂',
+      have exp.true x₁ e₁' ≠ exp.unop x₂ op₂ y₂ e₂', by contradiction,
+      show decidable (exp.true x₁ e₁' = exp.unop x₂ op₂ y₂ e₂'), from is_false this
+    ) (
+      assume x₂ op₂ y₂ z₂ e₂',
+      have exp.true x₁ e₁' ≠ exp.binop x₂ op₂ y₂ z₂ e₂', by contradiction,
+      show decidable (exp.true x₁ e₁' = exp.binop x₂ op₂ y₂ z₂ e₂'), from is_false this
+    ) (
+      assume x₂ y₂ z₂ e₂',
+      have exp.true x₁ e₁' ≠ exp.app x₂ y₂ z₂ e₂', by contradiction,
+      show decidable (exp.true x₁ e₁' = exp.app x₂ y₂ z₂ e₂'), from is_false this
+    ) (
+      assume x₂ e₂' e₂'',
+      have exp.true x₁ e₁' ≠ exp.ite x₂ e₂' e₂'', by contradiction,
+      show decidable (exp.true x₁ e₁' = exp.ite x₂ e₂' e₂''), from is_false this
+    ) (
+      assume x₂,
+      have exp.true x₁ e₁' ≠ exp.return x₂, by contradiction,
+      show decidable (exp.true x₁ e₁' = exp.return x₂), from is_false this
+    )
+  ) (
+    assume x₁ e₁',
+    assume : z = exp.false x₁ e₁',
+    have e₁_is_false: e₁ = exp.false x₁ e₁', from eq.trans h this,
+    show decidable (exp.false x₁ e₁' = e₂),
+    from exp.cases_on (λe₂, decidable (exp.false x₁ e₁' = e₂)) e₂ (
+      assume x₂ e₂',
+      have exp.false x₁ e₁' ≠ exp.true x₂ e₂', by contradiction,
+      show decidable (exp.false x₁ e₁' = exp.true x₂ e₂'), from is_false this
+    ) (
+      assume x₂ e₂',
+      have e₁'.sizeof < e₁.sizeof, from e₁_is_false.symm ▸ sizeof_exp_false,
+      have decidable (e₁' = e₂'), from exp.dec_eq e₁' e₂',
+      if h: (x₁ = x₂) ∧ (e₁' = e₂') then (
+        have exp.false x₁ e₁' = exp.false x₂ e₂',
+        from h.left ▸ h.right ▸ rfl,
+        show decidable (exp.false x₁ e₁' = exp.false x₂ e₂'),
+        from is_true this
+      ) else (
+        have exp.false x₁ e₁' ≠ exp.false x₂ e₂', from (
+          assume : exp.false x₁ e₁' = exp.false x₂ e₂',
+          show «false», from h (exp.false.inj this)
+        ),
+        show decidable (exp.false x₁ e₁' = exp.false x₂ e₂'),
+        from is_false this
+      )
+    ) (
+      assume x₂ n₂ e₂',
+      have exp.false x₁ e₁' ≠ exp.num x₂ n₂ e₂', by contradiction,
+      show decidable (exp.false x₁ e₁' = exp.num x₂ n₂ e₂'), from is_false this
+    ) (
+      assume f₂ x₂ R₂ S₂ e₂' e₂'',
+      have exp.false x₁ e₁' ≠ exp.func f₂ x₂ R₂ S₂ e₂' e₂'', by contradiction,
+      show decidable (exp.false x₁ e₁' = exp.func f₂ x₂ R₂ S₂ e₂' e₂''), from is_false this
+    ) (
+      assume x₂ op₂ y₂ e₂',
+      have exp.false x₁ e₁' ≠ exp.unop x₂ op₂ y₂ e₂', by contradiction,
+      show decidable (exp.false x₁ e₁' = exp.unop x₂ op₂ y₂ e₂'), from is_false this
+    ) (
+      assume x₂ op₂ y₂ z₂ e₂',
+      have exp.false x₁ e₁' ≠ exp.binop x₂ op₂ y₂ z₂ e₂', by contradiction,
+      show decidable (exp.false x₁ e₁' = exp.binop x₂ op₂ y₂ z₂ e₂'), from is_false this
+    ) (
+      assume x₂ y₂ z₂ e₂',
+      have exp.false x₁ e₁' ≠ exp.app x₂ y₂ z₂ e₂', by contradiction,
+      show decidable (exp.false x₁ e₁' = exp.app x₂ y₂ z₂ e₂'), from is_false this
+    ) (
+      assume x₂ e₂' e₂'',
+      have exp.false x₁ e₁' ≠ exp.ite x₂ e₂' e₂'', by contradiction,
+      show decidable (exp.false x₁ e₁' = exp.ite x₂ e₂' e₂''), from is_false this
+    ) (
+      assume x₂,
+      have exp.false x₁ e₁' ≠ exp.return x₂, by contradiction,
+      show decidable (exp.false x₁ e₁' = exp.return x₂), from is_false this
+    )
+  ) (
+    assume x₁ n₁ e₁',
+    assume : z = exp.num x₁ n₁ e₁',
+    have e₁_is_num: e₁ = exp.num x₁ n₁ e₁', from eq.trans h this,
+    show decidable (exp.num x₁ n₁ e₁' = e₂),
+    from exp.cases_on (λe₂, decidable (exp.num x₁ n₁ e₁' = e₂)) e₂ (
+      assume x₂ e₂',
+      have exp.num x₁ n₁ e₁' ≠ exp.true x₂ e₂', by contradiction,
+      show decidable (exp.num x₁ n₁ e₁' = exp.true x₂ e₂'), from is_false this
+    ) (
+      assume x₂ e₂',
+      have exp.num x₁ n₁ e₁' ≠ exp.false x₂ e₂', by contradiction,
+      show decidable (exp.num x₁ n₁ e₁' = exp.false x₂ e₂'), from is_false this
+    ) (
+      assume x₂ n₂ e₂',
+      have e₁'.sizeof < e₁.sizeof, from e₁_is_num.symm ▸ sizeof_exp_num,
+      have decidable (e₁' = e₂'), from exp.dec_eq e₁' e₂',
+      if h: (x₁ = x₂) ∧ (n₁ = n₂) ∧ (e₁' = e₂') then (
+        have exp.num x₁ n₁ e₁' = exp.num x₂ n₂ e₂',
+        from h.left ▸ h.right.left ▸ h.right.right ▸ rfl,
+        show decidable (exp.num x₁ n₁ e₁' = exp.num x₂ n₂ e₂'),
+        from is_true this
+      ) else (
+        have exp.num x₁ n₁ e₁' ≠ exp.num x₂ n₂ e₂', from (
+          assume : exp.num x₁ n₁ e₁' = exp.num x₂ n₂ e₂',
+          show «false», from h (exp.num.inj this)
+        ),
+        show decidable (exp.num x₁ n₁ e₁' = exp.num x₂ n₂ e₂'),
+        from is_false this
+      )
+    ) (
+      assume f₂ x₂ R₂ S₂ e₂' e₂'',
+      have exp.num x₁ n₁ e₁' ≠ exp.func f₂ x₂ R₂ S₂ e₂' e₂'', by contradiction,
+      show decidable (exp.num x₁ n₁ e₁' = exp.func f₂ x₂ R₂ S₂ e₂' e₂''), from is_false this
+    ) (
+      assume x₂ op₂ y₂ e₂',
+      have exp.num x₁ n₁ e₁' ≠ exp.unop x₂ op₂ y₂ e₂', by contradiction,
+      show decidable (exp.num x₁ n₁ e₁' = exp.unop x₂ op₂ y₂ e₂'), from is_false this
+    ) (
+      assume x₂ op₂ y₂ z₂ e₂',
+      have exp.num x₁ n₁ e₁' ≠ exp.binop x₂ op₂ y₂ z₂ e₂', by contradiction,
+      show decidable (exp.num x₁ n₁ e₁' = exp.binop x₂ op₂ y₂ z₂ e₂'), from is_false this
+    ) (
+      assume x₂ y₂ z₂ e₂',
+      have exp.num x₁ n₁ e₁' ≠ exp.app x₂ y₂ z₂ e₂', by contradiction,
+      show decidable (exp.num x₁ n₁ e₁' = exp.app x₂ y₂ z₂ e₂'), from is_false this
+    ) (
+      assume x₂ e₂' e₂'',
+      have exp.num x₁ n₁ e₁' ≠ exp.ite x₂ e₂' e₂'', by contradiction,
+      show decidable (exp.num x₁ n₁ e₁' = exp.ite x₂ e₂' e₂''), from is_false this
+    ) (
+      assume x₂,
+      have exp.num x₁ n₁ e₁' ≠ exp.return x₂, by contradiction,
+      show decidable (exp.num x₁ n₁ e₁' = exp.return x₂), from is_false this
+    )
+  ) (
+    assume f₁ x₁ R₁ S₁ e₁' e₁'',
+    assume : z = exp.func f₁ x₁ R₁ S₁ e₁' e₁'',
+    have e₁_is_func: e₁ = exp.func f₁ x₁ R₁ S₁ e₁' e₁'', from eq.trans h this,
+    show decidable (exp.func f₁ x₁ R₁ S₁ e₁' e₁'' = e₂),
+    from exp.cases_on (λe₂, decidable (exp.func f₁ x₁ R₁ S₁ e₁' e₁'' = e₂)) e₂ (
+      assume x₂ e₂',
+      have exp.func f₁ x₁ R₁ S₁ e₁' e₁'' ≠ exp.true x₂ e₂', by contradiction,
+      show decidable (exp.func f₁ x₁ R₁ S₁ e₁' e₁'' = exp.true x₂ e₂'), from is_false this
+    ) (
+      assume x₂ e₂',
+      have exp.func f₁ x₁ R₁ S₁ e₁' e₁'' ≠ exp.false x₂ e₂', by contradiction,
+      show decidable (exp.func f₁ x₁ R₁ S₁ e₁' e₁'' = exp.false x₂ e₂'), from is_false this
+    ) (
+      assume x₂ n₂ e₂',
+      have exp.func f₁ x₁ R₁ S₁ e₁' e₁'' ≠ exp.num x₂ n₂ e₂', by contradiction,
+      show decidable (exp.func f₁ x₁ R₁ S₁ e₁' e₁'' = exp.num x₂ n₂ e₂'), from is_false this
+    ) (
+      assume f₂ x₂ R₂ S₂ e₂' e₂'',
+      have R₁.sizeof < e₁.sizeof, from e₁_is_func.symm ▸ sizeof_exp_func_R,
+      have decidable (R₁ = R₂), from spec.dec_eq R₁ R₂,
+      have S₁.sizeof < e₁.sizeof, from e₁_is_func.symm ▸ sizeof_exp_func_S,
+      have decidable (S₁ = S₂), from spec.dec_eq S₁ S₂,
+      have e₁'.sizeof < e₁.sizeof, from e₁_is_func.symm ▸ sizeof_exp_func_e₁,
+      have decidable (e₁' = e₂'), from exp.dec_eq e₁' e₂',
+      have e₁''.sizeof < e₁.sizeof, from e₁_is_func.symm ▸ sizeof_exp_func_e₂,
+      have decidable (e₁'' = e₂''), from exp.dec_eq e₁'' e₂'',
+
+      if h: (f₁ = f₂) ∧ (x₁ = x₂) ∧ (R₁ = R₂) ∧ (S₁ = S₂) ∧ (e₁' = e₂') ∧ (e₁'' = e₂'') then (
+        have exp.func f₁ x₁ R₁ S₁ e₁' e₁'' = exp.func f₂ x₂ R₂ S₂ e₂' e₂'',
+        from h.left ▸ h.right.left ▸ h.right.right.left ▸ h.right.right.right.left ▸
+             h.right.right.right.right.left ▸ h.right.right.right.right.right ▸ rfl,
+        show decidable (exp.func f₁ x₁ R₁ S₁ e₁' e₁'' = exp.func f₂ x₂ R₂ S₂ e₂' e₂''),
+        from is_true this
+      ) else (
+        have exp.func f₁ x₁ R₁ S₁ e₁' e₁'' ≠ exp.func f₂ x₂ R₂ S₂ e₂' e₂'', from (
+          assume : exp.func f₁ x₁ R₁ S₁ e₁' e₁'' = exp.func f₂ x₂ R₂ S₂ e₂' e₂'',
+          show «false», from h (exp.func.inj this)
+        ),
+        show decidable (exp.func f₁ x₁ R₁ S₁ e₁' e₁'' = exp.func f₂ x₂ R₂ S₂ e₂' e₂''),
+        from is_false this
+      )
+    ) (
+      assume x₂ op₂ y₂ e₂',
+      have exp.func f₁ x₁ R₁ S₁ e₁' e₁'' ≠ exp.unop x₂ op₂ y₂ e₂', by contradiction,
+      show decidable (exp.func f₁ x₁ R₁ S₁ e₁' e₁'' = exp.unop x₂ op₂ y₂ e₂'), from is_false this
+    ) (
+      assume x₂ op₂ y₂ z₂ e₂',
+      have exp.func f₁ x₁ R₁ S₁ e₁' e₁'' ≠ exp.binop x₂ op₂ y₂ z₂ e₂', by contradiction,
+      show decidable (exp.func f₁ x₁ R₁ S₁ e₁' e₁'' = exp.binop x₂ op₂ y₂ z₂ e₂'), from is_false this
+    ) (
+      assume x₂ y₂ z₂ e₂',
+      have exp.func f₁ x₁ R₁ S₁ e₁' e₁'' ≠ exp.app x₂ y₂ z₂ e₂', by contradiction,
+      show decidable (exp.func f₁ x₁ R₁ S₁ e₁' e₁'' = exp.app x₂ y₂ z₂ e₂'), from is_false this
+    ) (
+      assume x₂ e₂' e₂'',
+      have exp.func f₁ x₁ R₁ S₁ e₁' e₁'' ≠ exp.ite x₂ e₂' e₂'', by contradiction,
+      show decidable (exp.func f₁ x₁ R₁ S₁ e₁' e₁'' = exp.ite x₂ e₂' e₂''), from is_false this
+    ) (
+      assume x₂,
+      have exp.func f₁ x₁ R₁ S₁ e₁' e₁'' ≠ exp.return x₂, by contradiction,
+      show decidable (exp.func f₁ x₁ R₁ S₁ e₁' e₁'' = exp.return x₂), from is_false this
+    )
+  ) (
+    assume x₁ op₁ y₁ e₁',
+    assume : z = exp.unop x₁ op₁ y₁ e₁',
+    have e₁_is_unop: e₁ = exp.unop x₁ op₁ y₁ e₁', from eq.trans h this,
+    show decidable (exp.unop x₁ op₁ y₁ e₁' = e₂),
+    from exp.cases_on (λe₂, decidable (exp.unop x₁ op₁ y₁ e₁' = e₂)) e₂ (
+      assume x₂ e₂',
+      have exp.unop x₁ op₁ y₁ e₁' ≠ exp.true x₂ e₂', by contradiction,
+      show decidable (exp.unop x₁ op₁ y₁ e₁' = exp.true x₂ e₂'), from is_false this
+    ) (
+      assume x₂ e₂',
+      have exp.unop x₁ op₁ y₁ e₁' ≠ exp.false x₂ e₂', by contradiction,
+      show decidable (exp.unop x₁ op₁ y₁ e₁' = exp.false x₂ e₂'), from is_false this
+    ) (
+      assume x₂ n₂ e₂',
+      have exp.unop x₁ op₁ y₁ e₁' ≠ exp.num x₂ n₂ e₂', by contradiction,
+      show decidable (exp.unop x₁ op₁ y₁ e₁' = exp.num x₂ n₂ e₂'), from is_false this
+    ) (
+      assume f₂ x₂ R₂ S₂ e₂' e₂'',
+      have exp.unop x₁ op₁ y₁ e₁' ≠ exp.func f₂ x₂ R₂ S₂ e₂' e₂'', by contradiction,
+      show decidable (exp.unop x₁ op₁ y₁ e₁' = exp.func f₂ x₂ R₂ S₂ e₂' e₂''), from is_false this
+    ) (
+      assume x₂ op₂ y₂ e₂',
+      have e₁'.sizeof < e₁.sizeof, from e₁_is_unop.symm ▸ sizeof_exp_unop,
+      have decidable (e₁' = e₂'), from exp.dec_eq e₁' e₂',
+      if h: (x₁ = x₂) ∧ (op₁ = op₂) ∧ (y₁ = y₂) ∧ (e₁' = e₂') then (
+        have exp.unop x₁ op₁ y₁ e₁' = exp.unop x₂ op₂ y₂ e₂',
+        from h.left ▸ h.right.left ▸ h.right.right.left ▸ h.right.right.right ▸ rfl,
+        show decidable (exp.unop x₁ op₁ y₁ e₁' = exp.unop x₂ op₂ y₂ e₂'),
+        from is_true this
+      ) else (
+        have exp.unop x₁ op₁ y₁ e₁' ≠ exp.unop x₂ op₂ y₂ e₂', from (
+          assume : exp.unop x₁ op₁ y₁ e₁' = exp.unop x₂ op₂ y₂ e₂',
+          show «false», from h (exp.unop.inj this)
+        ),
+        show decidable (exp.unop x₁ op₁ y₁ e₁' = exp.unop x₂ op₂ y₂ e₂'),
+        from is_false this
+      )
+    ) (
+      assume x₂ op₂ y₂ z₂ e₂',
+      have exp.unop x₁ op₁ y₁ e₁' ≠ exp.binop x₂ op₂ y₂ z₂ e₂', by contradiction,
+      show decidable (exp.unop x₁ op₁ y₁ e₁' = exp.binop x₂ op₂ y₂ z₂ e₂'), from is_false this
+    ) (
+      assume x₂ y₂ z₂ e₂',
+      have exp.unop x₁ op₁ y₁ e₁' ≠ exp.app x₂ y₂ z₂ e₂', by contradiction,
+      show decidable (exp.unop x₁ op₁ y₁ e₁' = exp.app x₂ y₂ z₂ e₂'), from is_false this
+    ) (
+      assume x₂ e₂' e₂'',
+      have exp.unop x₁ op₁ y₁ e₁' ≠ exp.ite x₂ e₂' e₂'', by contradiction,
+      show decidable (exp.unop x₁ op₁ y₁ e₁' = exp.ite x₂ e₂' e₂''), from is_false this
+    ) (
+      assume x₂,
+      have exp.unop x₁ op₁ y₁ e₁' ≠ exp.return x₂, by contradiction,
+      show decidable (exp.unop x₁ op₁ y₁ e₁' = exp.return x₂), from is_false this
+    )
+  ) (
+    assume x₁ op₁ y₁ z₁ e₁',
+    assume : z = exp.binop x₁ op₁ y₁ z₁ e₁',
+    have e₁_is_binop: e₁ = exp.binop x₁ op₁ y₁ z₁ e₁', from eq.trans h this,
+    show decidable (exp.binop x₁ op₁ y₁ z₁ e₁' = e₂),
+    from exp.cases_on (λe₂, decidable (exp.binop x₁ op₁ y₁ z₁ e₁' = e₂)) e₂ (
+      assume x₂ e₂',
+      have exp.binop x₁ op₁ y₁ z₁ e₁' ≠ exp.true x₂ e₂', by contradiction,
+      show decidable (exp.binop x₁ op₁ y₁ z₁ e₁' = exp.true x₂ e₂'), from is_false this
+    ) (
+      assume x₂ e₂',
+      have exp.binop x₁ op₁ y₁ z₁ e₁' ≠ exp.false x₂ e₂', by contradiction,
+      show decidable (exp.binop x₁ op₁ y₁ z₁ e₁' = exp.false x₂ e₂'), from is_false this
+    ) (
+      assume x₂ n₂ e₂',
+      have exp.binop x₁ op₁ y₁ z₁ e₁' ≠ exp.num x₂ n₂ e₂', by contradiction,
+      show decidable (exp.binop x₁ op₁ y₁ z₁ e₁' = exp.num x₂ n₂ e₂'), from is_false this
+    ) (
+      assume f₂ x₂ R₂ S₂ e₂' e₂'',
+      have exp.binop x₁ op₁ y₁ z₁ e₁' ≠ exp.func f₂ x₂ R₂ S₂ e₂' e₂'', by contradiction,
+      show decidable (exp.binop x₁ op₁ y₁ z₁ e₁' = exp.func f₂ x₂ R₂ S₂ e₂' e₂''), from is_false this
+    ) (
+      assume x₂ op₂ y₂ e₂',
+      have exp.binop x₁ op₁ y₁ z₁ e₁' ≠ exp.unop x₂ op₂ y₂ e₂', by contradiction,
+      show decidable (exp.binop x₁ op₁ y₁ z₁ e₁' = exp.unop x₂ op₂ y₂ e₂'), from is_false this
+    ) (
+      assume x₂ op₂ y₂ z₂ e₂',
+      have e₁'.sizeof < e₁.sizeof, from e₁_is_binop.symm ▸ sizeof_exp_binop,
+      have decidable (e₁' = e₂'), from exp.dec_eq e₁' e₂',
+      if h: (x₁ = x₂) ∧ (op₁ = op₂) ∧ (y₁ = y₂) ∧ (z₁ = z₂) ∧ (e₁' = e₂') then (
+        have exp.binop x₁ op₁ y₁ z₁ e₁' = exp.binop x₂ op₂ y₂ z₂ e₂',
+        from h.left ▸ h.right.left ▸ h.right.right.left ▸ h.right.right.right.left ▸
+             h.right.right.right.right ▸ rfl,
+        show decidable (exp.binop x₁ op₁ y₁ z₁ e₁' = exp.binop x₂ op₂ y₂ z₂ e₂'),
+        from is_true this
+      ) else (
+        have exp.binop x₁ op₁ y₁ z₁ e₁' ≠ exp.binop x₂ op₂ y₂ z₂ e₂', from (
+          assume : exp.binop x₁ op₁ y₁ z₁ e₁' = exp.binop x₂ op₂ y₂ z₂ e₂',
+          show «false», from h (exp.binop.inj this)
+        ),
+        show decidable (exp.binop x₁ op₁ y₁ z₁ e₁' = exp.binop x₂ op₂ y₂ z₂ e₂'),
+        from is_false this
+      )
+    ) (
+      assume x₂ y₂ z₂ e₂',
+      have exp.binop x₁ op₁ y₁ z₁ e₁' ≠ exp.app x₂ y₂ z₂ e₂', by contradiction,
+      show decidable (exp.binop x₁ op₁ y₁ z₁ e₁' = exp.app x₂ y₂ z₂ e₂'), from is_false this
+    ) (
+      assume x₂ e₂' e₂'',
+      have exp.binop x₁ op₁ y₁ z₁ e₁' ≠ exp.ite x₂ e₂' e₂'', by contradiction,
+      show decidable (exp.binop x₁ op₁ y₁ z₁ e₁' = exp.ite x₂ e₂' e₂''), from is_false this
+    ) (
+      assume x₂,
+      have exp.binop x₁ op₁ y₁ z₁ e₁' ≠ exp.return x₂, by contradiction,
+      show decidable (exp.binop x₁ op₁ y₁ z₁ e₁' = exp.return x₂), from is_false this
+    )
+  ) (
+    assume x₁ y₁ z₁ e₁',
+    assume : z = exp.app x₁ y₁ z₁ e₁',
+    have e₁_is_app: e₁ = exp.app x₁ y₁ z₁ e₁', from eq.trans h this,
+    show decidable (exp.app x₁ y₁ z₁ e₁' = e₂),
+    from exp.cases_on (λe₂, decidable (exp.app x₁ y₁ z₁ e₁' = e₂)) e₂ (
+      assume x₂ e₂',
+      have exp.app x₁ y₁ z₁ e₁' ≠ exp.true x₂ e₂', by contradiction,
+      show decidable (exp.app x₁ y₁ z₁ e₁' = exp.true x₂ e₂'), from is_false this
+    ) (
+      assume x₂ e₂',
+      have exp.app x₁ y₁ z₁ e₁' ≠ exp.false x₂ e₂', by contradiction,
+      show decidable (exp.app x₁ y₁ z₁ e₁' = exp.false x₂ e₂'), from is_false this
+    ) (
+      assume x₂ n₂ e₂',
+      have exp.app x₁ y₁ z₁ e₁' ≠ exp.num x₂ n₂ e₂', by contradiction,
+      show decidable (exp.app x₁ y₁ z₁ e₁' = exp.num x₂ n₂ e₂'), from is_false this
+    ) (
+      assume f₂ x₂ R₂ S₂ e₂' e₂'',
+      have exp.app x₁ y₁ z₁ e₁' ≠ exp.func f₂ x₂ R₂ S₂ e₂' e₂'', by contradiction,
+      show decidable (exp.app x₁ y₁ z₁ e₁' = exp.func f₂ x₂ R₂ S₂ e₂' e₂''), from is_false this
+    ) (
+      assume x₂ op₂ y₂ e₂',
+      have exp.app x₁ y₁ z₁ e₁' ≠ exp.unop x₂ op₂ y₂ e₂', by contradiction,
+      show decidable (exp.app x₁ y₁ z₁ e₁' = exp.unop x₂ op₂ y₂ e₂'), from is_false this
+    ) (
+      assume x₂ op₂ y₂ z₂ e₂',
+      have exp.app x₁ y₁ z₁ e₁' ≠ exp.binop x₂ op₂ y₂ z₂ e₂', by contradiction,
+      show decidable (exp.app x₁ y₁ z₁ e₁' = exp.binop x₂ op₂ y₂ z₂ e₂'), from is_false this
+    ) (
+      assume x₂ y₂ z₂ e₂',
+      have e₁'.sizeof < e₁.sizeof, from e₁_is_app.symm ▸ sizeof_exp_app,
+      have decidable (e₁' = e₂'), from exp.dec_eq e₁' e₂',
+      if h: (x₁ = x₂) ∧ (y₁ = y₂) ∧ (z₁ = z₂) ∧ (e₁' = e₂') then (
+        have exp.app x₁ y₁ z₁ e₁' = exp.app x₂ y₂ z₂ e₂',
+        from h.left ▸ h.right.left ▸ h.right.right.left ▸ h.right.right.right ▸ rfl,
+        show decidable (exp.app x₁ y₁ z₁ e₁' = exp.app x₂ y₂ z₂ e₂'),
+        from is_true this
+      ) else (
+        have exp.app x₁ y₁ z₁ e₁' ≠ exp.app x₂ y₂ z₂ e₂', from (
+          assume : exp.app x₁ y₁ z₁ e₁' = exp.app x₂ y₂ z₂ e₂',
+          show «false», from h (exp.app.inj this)
+        ),
+        show decidable (exp.app x₁ y₁ z₁ e₁' = exp.app x₂ y₂ z₂ e₂'),
+        from is_false this
+      )
+    ) (
+      assume x₂ e₂' e₂'',
+      have exp.app x₁ y₁ z₁ e₁' ≠ exp.ite x₂ e₂' e₂'', by contradiction,
+      show decidable (exp.app x₁ y₁ z₁ e₁' = exp.ite x₂ e₂' e₂''), from is_false this
+    ) (
+      assume x₂,
+      have exp.app x₁ y₁ z₁ e₁' ≠ exp.return x₂, by contradiction,
+      show decidable (exp.app x₁ y₁ z₁ e₁' = exp.return x₂), from is_false this
+    )
+  ) (
+    assume x₁ e₁' e₁'',
+    assume : z = exp.ite x₁ e₁' e₁'',
+    have e₁_is_ite: e₁ = exp.ite x₁ e₁' e₁'', from eq.trans h this,
+    show decidable (exp.ite x₁ e₁' e₁'' = e₂),
+    from exp.cases_on (λe₂, decidable (exp.ite x₁ e₁' e₁'' = e₂)) e₂ (
+      assume x₂ e₂',
+      have exp.ite x₁ e₁' e₁'' ≠ exp.true x₂ e₂', by contradiction,
+      show decidable (exp.ite x₁ e₁' e₁'' = exp.true x₂ e₂'), from is_false this
+    ) (
+      assume x₂ e₂',
+      have exp.ite x₁ e₁' e₁'' ≠ exp.false x₂ e₂', by contradiction,
+      show decidable (exp.ite x₁ e₁' e₁'' = exp.false x₂ e₂'), from is_false this
+    ) (
+      assume x₂ n₂ e₂',
+      have exp.ite x₁ e₁' e₁'' ≠ exp.num x₂ n₂ e₂', by contradiction,
+      show decidable (exp.ite x₁ e₁' e₁'' = exp.num x₂ n₂ e₂'), from is_false this
+    ) (
+      assume f₂ x₂ R₂ S₂ e₂' e₂'',
+      have exp.ite x₁ e₁' e₁'' ≠ exp.func f₂ x₂ R₂ S₂ e₂' e₂'', by contradiction,
+      show decidable (exp.ite x₁ e₁' e₁'' = exp.func f₂ x₂ R₂ S₂ e₂' e₂''), from is_false this
+    ) (
+      assume x₂ op₂ y₂ e₂',
+      have exp.ite x₁ e₁' e₁'' ≠ exp.unop x₂ op₂ y₂ e₂', by contradiction,
+      show decidable (exp.ite x₁ e₁' e₁'' = exp.unop x₂ op₂ y₂ e₂'), from is_false this
+    ) (
+      assume x₂ op₂ y₂ z₂ e₂',
+      have exp.ite x₁ e₁' e₁'' ≠ exp.binop x₂ op₂ y₂ z₂ e₂', by contradiction,
+      show decidable (exp.ite x₁ e₁' e₁'' = exp.binop x₂ op₂ y₂ z₂ e₂'), from is_false this
+    ) (
+      assume x₂ y₂ z₂ e₂',
+      have exp.ite x₁ e₁' e₁'' ≠ exp.app x₂ y₂ z₂ e₂', by contradiction,
+      show decidable (exp.ite x₁ e₁' e₁'' = exp.app x₂ y₂ z₂ e₂'), from is_false this
+    ) (
+      assume x₂ e₂' e₂'',
+      have e₁'.sizeof < e₁.sizeof, from e₁_is_ite.symm ▸ sizeof_exp_ite_e₁,
+      have decidable (e₁' = e₂'), from exp.dec_eq e₁' e₂',
+      have e₁''.sizeof < e₁.sizeof, from e₁_is_ite.symm ▸ sizeof_exp_ite_e₂,
+      have decidable (e₁'' = e₂''), from exp.dec_eq e₁'' e₂'',
+      if h: (x₁ = x₂) ∧ (e₁' = e₂') ∧ (e₁'' = e₂'') then (
+        have exp.ite x₁ e₁' e₁'' = exp.ite x₂ e₂' e₂'',
+        from h.left ▸ h.right.left ▸ h.right.right ▸ rfl,
+        show decidable (exp.ite x₁ e₁' e₁'' = exp.ite x₂ e₂' e₂''),
+        from is_true this
+      ) else (
+        have exp.ite x₁ e₁' e₁'' ≠ exp.ite x₂ e₂' e₂'', from (
+          assume : exp.ite x₁ e₁' e₁'' = exp.ite x₂ e₂' e₂'',
+          show «false», from h (exp.ite.inj this)
+        ),
+        show decidable (exp.ite x₁ e₁' e₁'' = exp.ite x₂ e₂' e₂''),
+        from is_false this
+      )
+    ) (
+      assume x₂,
+      have exp.ite x₁ e₁' e₁'' ≠ exp.return x₂, by contradiction,
+      show decidable (exp.ite x₁ e₁' e₁'' = exp.return x₂), from is_false this
+    )
+  ) (
+    assume x₁,
+    assume : z = exp.return x₁,
+    have e₁_is_tru: e₁ = exp.return x₁, from eq.trans h this,
+    show decidable (exp.return x₁ = e₂),
+    from exp.cases_on (λe₂, decidable (exp.return x₁ = e₂)) e₂ (
+      assume x₂ e₂',
+      have exp.return x₁ ≠ exp.true x₂ e₂', by contradiction,
+      show decidable (exp.return x₁ = exp.true x₂ e₂'), from is_false this
+    ) (
+      assume x₂ e₂',
+      have exp.return x₁ ≠ exp.false x₂ e₂', by contradiction,
+      show decidable (exp.return x₁ = exp.false x₂ e₂'), from is_false this
+    ) (
+      assume x₂ n₂ e₂',
+      have exp.return x₁ ≠ exp.num x₂ n₂ e₂', by contradiction,
+      show decidable (exp.return x₁ = exp.num x₂ n₂ e₂'), from is_false this
+    ) (
+      assume f₂ x₂ R₂ S₂ e₂' e₂'',
+      have exp.return x₁ ≠ exp.func f₂ x₂ R₂ S₂ e₂' e₂'', by contradiction,
+      show decidable (exp.return x₁ = exp.func f₂ x₂ R₂ S₂ e₂' e₂''), from is_false this
+    ) (
+      assume x₂ op₂ y₂ e₂',
+      have exp.return x₁ ≠ exp.unop x₂ op₂ y₂ e₂', by contradiction,
+      show decidable (exp.return x₁ = exp.unop x₂ op₂ y₂ e₂'), from is_false this
+    ) (
+      assume x₂ op₂ y₂ z₂ e₂',
+      have exp.return x₁ ≠ exp.binop x₂ op₂ y₂ z₂ e₂', by contradiction,
+      show decidable (exp.return x₁ = exp.binop x₂ op₂ y₂ z₂ e₂'), from is_false this
+    ) (
+      assume x₂ y₂ z₂ e₂',
+      have exp.return x₁ ≠ exp.app x₂ y₂ z₂ e₂', by contradiction,
+      show decidable (exp.return x₁ = exp.app x₂ y₂ z₂ e₂'), from is_false this
+    ) (
+      assume x₂ e₂' e₂'',
+      have exp.return x₁ ≠ exp.ite x₂ e₂' e₂'', by contradiction,
+      show decidable (exp.return x₁ = exp.ite x₂ e₂' e₂''), from is_false this
+    ) (
+      assume x₂,
+      if h: x₁ = x₂ then (
+        have exp.return x₁ = exp.return x₂, from h ▸ rfl,
+        show decidable (exp.return x₁ = exp.return x₂),
+        from is_true this
+      ) else (
+        have exp.return x₁ ≠ exp.return x₂, from (
+          assume : exp.return x₁ = exp.return x₂,
+          show «false», from h (exp.return.inj this)
+        ),
+        show decidable (exp.return x₁ = exp.return x₂),
+        from is_false this
+      )
+    )
+  ) rfl
+
+with term.dec_eq : ∀ (t₁ t₂: term), decidable (t₁ = t₂)
+| t₁ t₂ :=
+  let z := t₁ in
+  have h: z = t₁, from rfl,
+  term.cases_on (λt₁, (z = t₁) → decidable (t₁ = t₂)) t₁ (
+    assume v₁,
+    assume : z = term.value v₁,
+    have t₁_id: t₁ = term.value v₁, from eq.trans h this,
+    show decidable (term.value v₁ = t₂),
+    from term.cases_on (λt₂, decidable (term.value v₁ = t₂)) t₂ (
+      assume v₂,
+      have v₁.sizeof < t₁.sizeof, from t₁_id.symm ▸ sizeof_term_value,
+      have decidable (v₁ = v₂), from value.dec_eq v₁ v₂,
+      if h: v₁ = v₂ then (
+        have term.value v₁ = term.value v₂, from h ▸ rfl,
+        show decidable (term.value v₁ = term.value v₂),
+        from is_true this
+      ) else (
+        have term.value v₁ ≠ term.value v₂, from (
+          assume : term.value v₁ = term.value v₂,
+          show «false», from h (term.value.inj this)
+        ),
+        show decidable (term.value v₁ = term.value v₂),
+        from is_false this
+      )
+    ) (
+      assume x₂,
+      have term.value v₁ ≠ term.var x₂, by contradiction,
+      show decidable (term.value v₁ = term.var x₂), from is_false this
+    ) (
+      assume op₂ t₂',
+      have term.value v₁ ≠ term.unop op₂ t₂', by contradiction,
+      show decidable (term.value v₁ = term.unop op₂ t₂'), from is_false this
+    ) (
+      assume op₂ t₂' t₂'',
+      have term.value v₁ ≠ term.binop op₂ t₂' t₂'', by contradiction,
+      show decidable (term.value v₁ = term.binop op₂ t₂' t₂''), from is_false this
+    ) (
+      assume t₂' t₂'',
+      have term.value v₁ ≠ term.app t₂' t₂'', by contradiction,
+      show decidable (term.value v₁ = term.app t₂' t₂''), from is_false this
+    )
+  ) (
+    assume x₁,
+    assume : z = term.var x₁,
+    have t₁_id: t₁ = term.var x₁, from eq.trans h this,
+    show decidable (term.var x₁ = t₂),
+    from term.cases_on (λt₂, decidable (term.var x₁ = t₂)) t₂ (
+      assume v₂,
+      have term.var x₁ ≠ term.value v₂, by contradiction,
+      show decidable (term.var x₁ = term.value v₂), from is_false this
+    ) (
+      assume x₂,
+      if h: x₁ = x₂ then (
+        have term.var x₁ = term.var x₂, from h ▸ rfl,
+        show decidable (term.var x₁ = term.var x₂),
+        from is_true this
+      ) else (
+        have term.var x₁ ≠ term.var x₂, from (
+          assume : term.var x₁ = term.var x₂,
+          show «false», from h (term.var.inj this)
+        ),
+        show decidable (term.var x₁ = term.var x₂),
+        from is_false this
+      )
+    ) (
+      assume op₂ t₂',
+      have term.var x₁ ≠ term.unop op₂ t₂', by contradiction,
+      show decidable (term.var x₁ = term.unop op₂ t₂'), from is_false this
+    ) (
+      assume op₂ t₂' t₂'',
+      have term.var x₁ ≠ term.binop op₂ t₂' t₂'', by contradiction,
+      show decidable (term.var x₁ = term.binop op₂ t₂' t₂''), from is_false this
+    ) (
+      assume t₂' t₂'',
+      have term.var x₁ ≠ term.app t₂' t₂'', by contradiction,
+      show decidable (term.var x₁ = term.app t₂' t₂''), from is_false this
+    )
+  ) (
+    assume op₁ t₁',
+    assume : z = term.unop op₁ t₁',
+    have t₁_id: t₁ = term.unop op₁ t₁', from eq.trans h this,
+    show decidable (term.unop op₁ t₁' = t₂),
+    from term.cases_on (λt₂, decidable (term.unop op₁ t₁' = t₂)) t₂ (
+      assume v₂,
+      have term.unop op₁ t₁' ≠ term.value v₂, by contradiction,
+      show decidable (term.unop op₁ t₁' = term.value v₂), from is_false this
+    ) (
+      assume x₂,
+      have term.unop op₁ t₁' ≠ term.var x₂, by contradiction,
+      show decidable (term.unop op₁ t₁' = term.var x₂), from is_false this
+    ) (
+      assume op₂ t₂',
+      have t₁'.sizeof < t₁.sizeof, from t₁_id.symm ▸ sizeof_term_unop,
+      have decidable (t₁' = t₂'), from term.dec_eq t₁' t₂',
+      if h: (op₁ = op₂) ∧ (t₁' = t₂') then (
+        have term.unop op₁ t₁' = term.unop op₂ t₂',
+        from h.left ▸ h.right ▸ rfl,
+        show decidable (term.unop op₁ t₁' = term.unop op₂ t₂'),
+        from is_true this
+      ) else (
+        have term.unop op₁ t₁' ≠ term.unop op₂ t₂', from (
+          assume : term.unop op₁ t₁' = term.unop op₂ t₂',
+          show «false», from h (term.unop.inj this)
+        ),
+        show decidable (term.unop op₁ t₁' = term.unop op₂ t₂'),
+        from is_false this
+      )
+    ) (
+      assume op₂ t₂' t₂'',
+      have term.unop op₁ t₁' ≠ term.binop op₂ t₂' t₂'', by contradiction,
+      show decidable (term.unop op₁ t₁' = term.binop op₂ t₂' t₂''), from is_false this
+    ) (
+      assume t₂' t₂'',
+      have term.unop op₁ t₁' ≠ term.app t₂' t₂'', by contradiction,
+      show decidable (term.unop op₁ t₁' = term.app t₂' t₂''), from is_false this
+    )
+  ) (
+    assume op₁ t₁' t₁'',
+    assume : z = term.binop op₁ t₁' t₁'',
+    have t₁_id: t₁ = term.binop op₁ t₁' t₁'', from eq.trans h this,
+    show decidable (term.binop op₁ t₁' t₁'' = t₂),
+    from term.cases_on (λt₂, decidable (term.binop op₁ t₁' t₁'' = t₂)) t₂ (
+      assume v₂,
+      have term.binop op₁ t₁' t₁'' ≠ term.value v₂, by contradiction,
+      show decidable (term.binop op₁ t₁' t₁'' = term.value v₂), from is_false this
+    ) (
+      assume x₂,
+      have term.binop op₁ t₁' t₁'' ≠ term.var x₂, by contradiction,
+      show decidable (term.binop op₁ t₁' t₁'' = term.var x₂), from is_false this
+    ) (
+      assume op₂ t₂',
+      have term.binop op₁ t₁' t₁'' ≠ term.unop op₂ t₂', by contradiction,
+      show decidable (term.binop op₁ t₁' t₁'' = term.unop op₂ t₂'), from is_false this
+    ) (
+      assume op₂ t₂' t₂'',
+      have t₁'.sizeof < t₁.sizeof, from t₁_id.symm ▸ sizeof_term_binop₁,
+      have decidable (t₁' = t₂'), from term.dec_eq t₁' t₂',
+      have t₁''.sizeof < t₁.sizeof, from t₁_id.symm ▸ sizeof_term_binop₂,
+      have decidable (t₁'' = t₂''), from term.dec_eq t₁'' t₂'',
+      if h: (op₁ = op₂) ∧ (t₁' = t₂') ∧ (t₁'' = t₂'') then (
+        have term.binop op₁ t₁' t₁'' = term.binop op₂ t₂' t₂'',
+        from h.left ▸ h.right.left ▸ h.right.right ▸ rfl,
+        show decidable (term.binop op₁ t₁' t₁'' = term.binop op₂ t₂' t₂''),
+        from is_true this
+      ) else (
+        have term.binop op₁ t₁' t₁'' ≠ term.binop op₂ t₂' t₂'', from (
+          assume : term.binop op₁ t₁' t₁'' = term.binop op₂ t₂' t₂'',
+          show «false», from h (term.binop.inj this)
+        ),
+        show decidable (term.binop op₁ t₁' t₁'' = term.binop op₂ t₂' t₂''),
+        from is_false this
+      )
+    ) (
+      assume t₂' t₂'',
+      have term.binop op₁ t₁' t₁'' ≠ term.app t₂' t₂'', by contradiction,
+      show decidable (term.binop op₁ t₁' t₁'' = term.app t₂' t₂''), from is_false this
+    )
+  ) (
+    assume t₁' t₁'',
+    assume : z = term.app t₁' t₁'',
+    have t₁_id: t₁ = term.app t₁' t₁'', from eq.trans h this,
+    show decidable (term.app t₁' t₁'' = t₂),
+    from term.cases_on (λt₂, decidable (term.app t₁' t₁'' = t₂)) t₂ (
+      assume v₂,
+      have term.app t₁' t₁'' ≠ term.value v₂, by contradiction,
+      show decidable (term.app t₁' t₁'' = term.value v₂), from is_false this
+    ) (
+      assume x₂,
+      have term.app t₁' t₁'' ≠ term.var x₂, by contradiction,
+      show decidable (term.app t₁' t₁'' = term.var x₂), from is_false this
+    ) (
+      assume op₂ t₂',
+      have term.app t₁' t₁'' ≠ term.unop op₂ t₂', by contradiction,
+      show decidable (term.app t₁' t₁'' = term.unop op₂ t₂'), from is_false this
+    ) (
+      assume op₂ t₂' t₂'',
+      have term.app t₁' t₁'' ≠ term.binop op₂ t₂' t₂'', by contradiction,
+      show decidable (term.app t₁' t₁'' = term.binop op₂ t₂' t₂''), from is_false this
+    ) (
+      assume t₂' t₂'',
+      have t₁'.sizeof < t₁.sizeof, from t₁_id.symm ▸ sizeof_term_app₁,
+      have decidable (t₁' = t₂'), from term.dec_eq t₁' t₂',
+      have t₁''.sizeof < t₁.sizeof, from t₁_id.symm ▸ sizeof_term_app₂,
+      have decidable (t₁'' = t₂''), from term.dec_eq t₁'' t₂'',
+      if h: (t₁' = t₂') ∧ (t₁'' = t₂'') then (
+        have term.app t₁' t₁'' = term.app t₂' t₂'',
+        from h.left ▸ h.right ▸ rfl,
+        show decidable (term.app t₁' t₁'' = term.app t₂' t₂''),
+        from is_true this
+      ) else (
+        have term.app t₁' t₁'' ≠ term.app t₂' t₂'', from (
+          assume : term.app t₁' t₁'' = term.app t₂' t₂'',
+          show «false», from h (term.app.inj this)
+        ),
+        show decidable (term.app t₁' t₁'' = term.app t₂' t₂''),
+        from is_false this
+      )
+    )
+  ) rfl
+
+with spec.dec_eq : ∀ (R₁ R₂: spec), decidable (R₁ = R₂)
+| R₁ R₂ :=
+  let z := R₁ in
+  have h: z = R₁, from rfl,
+  spec.cases_on (λR₁, (z = R₁) → decidable (R₁ = R₂)) R₁ (
+    assume t₁,
+    assume : z = spec.term t₁,
+    have R₁_id: R₁ = spec.term t₁, from eq.trans h this,
+    show decidable (spec.term t₁ = R₂),
+    from spec.cases_on (λR₂, decidable (spec.term t₁ = R₂)) R₂ (
+      assume t₂,
+      have t₁.sizeof < R₁.sizeof, from R₁_id.symm ▸ sizeof_spec_term,
+      have decidable (t₁ = t₂), from term.dec_eq t₁ t₂,
+      if h: t₁ = t₂ then (
+        have spec.term t₁ = spec.term t₂, from h ▸ rfl,
+        show decidable (spec.term t₁ = spec.term t₂),
+        from is_true this
+      ) else (
+        have spec.term t₁ ≠ spec.term t₂, from (
+          assume : spec.term t₁ = spec.term t₂,
+          show «false», from h (spec.term.inj this)
+        ),
+        show decidable (spec.term t₁ = spec.term t₂),
+        from is_false this
+      )
+    ) (
+      assume S₂,
+      have spec.term t₁ ≠ spec.not S₂, by contradiction,
+      show decidable (spec.term t₁ = spec.not S₂), from is_false this
+    ) (
+      assume S₂ S₂',
+      have spec.term t₁ ≠ spec.and S₂ S₂', by contradiction,
+      show decidable (spec.term t₁ = spec.and S₂ S₂'), from is_false this
+    ) (
+      assume S₂ S₂',
+      have spec.term t₁ ≠ spec.or S₂ S₂', by contradiction,
+      show decidable (spec.term t₁ = spec.or S₂ S₂'), from is_false this
+    ) (
+      assume t₂ x₂ S₂ S₂',
+      have spec.term t₁ ≠ spec.func t₂ x₂ S₂ S₂', by contradiction,
+      show decidable (spec.term t₁ = spec.func t₂ x₂ S₂ S₂'), from is_false this
+    )
+  ) (
+    assume S₁,
+    assume : z = spec.not S₁,
+    have R₁_id: R₁ = spec.not S₁, from eq.trans h this,
+    show decidable (spec.not S₁ = R₂),
+    from spec.cases_on (λR₂, decidable (spec.not S₁ = R₂)) R₂ (
+      assume t₂,
+      have spec.not S₁ ≠ spec.term t₂, by contradiction,
+      show decidable (spec.not S₁ = spec.term t₂), from is_false this
+    ) (
+      assume S₂,
+      have S₁.sizeof < R₁.sizeof, from R₁_id.symm ▸ sizeof_spec_not,
+      have decidable (S₁ = S₂), from spec.dec_eq S₁ S₂,
+      if h: S₁ = S₂ then (
+        have spec.not S₁ = spec.not S₂, from h ▸ rfl,
+        show decidable (spec.not S₁ = spec.not S₂),
+        from is_true this
+      ) else (
+        have spec.not S₁ ≠ spec.not S₂, from (
+          assume : spec.not S₁ = spec.not S₂,
+          show «false», from h (spec.not.inj this)
+        ),
+        show decidable (spec.not S₁ = spec.not S₂),
+        from is_false this
+      )
+    ) (
+      assume S₂ S₂',
+      have spec.not S₁ ≠ spec.and S₂ S₂', by contradiction,
+      show decidable (spec.not S₁ = spec.and S₂ S₂'), from is_false this
+    ) (
+      assume S₂ S₂',
+      have spec.not S₁ ≠ spec.or S₂ S₂', by contradiction,
+      show decidable (spec.not S₁ = spec.or S₂ S₂'), from is_false this
+    ) (
+      assume t₂ x₂ S₂ S₂',
+      have spec.not S₁ ≠ spec.func t₂ x₂ S₂ S₂', by contradiction,
+      show decidable (spec.not S₁ = spec.func t₂ x₂ S₂ S₂'), from is_false this
+    )
+  ) (
+    assume S₁ S₁',
+    assume : z = spec.and S₁ S₁',
+    have R₁_id: R₁ = spec.and S₁ S₁', from eq.trans h this,
+    show decidable (spec.and S₁ S₁' = R₂),
+    from spec.cases_on (λR₂, decidable (spec.and S₁ S₁' = R₂)) R₂ (
+      assume t₂,
+      have spec.and S₁ S₁' ≠ spec.term t₂, by contradiction,
+      show decidable (spec.and S₁ S₁' = spec.term t₂), from is_false this
+    ) (
+      assume S₂,
+      have spec.and S₁ S₁' ≠ spec.not S₂, by contradiction,
+      show decidable (spec.and S₁ S₁' = spec.not S₂), from is_false this
+    ) (
+      assume S₂ S₂',
+      have S₁.sizeof < R₁.sizeof, from R₁_id.symm ▸ sizeof_spec_and₁,
+      have decidable (S₁ = S₂), from spec.dec_eq S₁ S₂,
+      have S₁'.sizeof < R₁.sizeof, from R₁_id.symm ▸ sizeof_spec_and₂,
+      have decidable (S₁' = S₂'), from spec.dec_eq S₁' S₂',
+      if h: (S₁ = S₂) ∧ (S₁' = S₂') then (
+        have spec.and S₁ S₁' = spec.and S₂ S₂',
+        from h.left ▸ h.right ▸ rfl,
+        show decidable (spec.and S₁ S₁' = spec.and S₂ S₂'),
+        from is_true this
+      ) else (
+        have spec.and S₁ S₁' ≠ spec.and S₂ S₂', from (
+          assume : spec.and S₁ S₁' = spec.and S₂ S₂',
+          show «false», from h (spec.and.inj this)
+        ),
+        show decidable (spec.and S₁ S₁' = spec.and S₂ S₂'),
+        from is_false this
+      )
+    ) (
+      assume S₂ S₂',
+      have spec.and S₁ S₁' ≠ spec.or S₂ S₂', by contradiction,
+      show decidable (spec.and S₁ S₁' = spec.or S₂ S₂'), from is_false this
+    ) (
+      assume t₂ x₂ S₂ S₂',
+      have spec.and S₁ S₁' ≠ spec.func t₂ x₂ S₂ S₂', by contradiction,
+      show decidable (spec.and S₁ S₁' = spec.func t₂ x₂ S₂ S₂'), from is_false this
+    )
+  ) (
+    assume S₁ S₁',
+    assume : z = spec.or S₁ S₁',
+    have R₁_id: R₁ = spec.or S₁ S₁', from eq.trans h this,
+    show decidable (spec.or S₁ S₁' = R₂),
+    from spec.cases_on (λR₂, decidable (spec.or S₁ S₁' = R₂)) R₂ (
+      assume t₂,
+      have spec.or S₁ S₁' ≠ spec.term t₂, by contradiction,
+      show decidable (spec.or S₁ S₁' = spec.term t₂), from is_false this
+    ) (
+      assume S₂,
+      have spec.or S₁ S₁' ≠ spec.not S₂, by contradiction,
+      show decidable (spec.or S₁ S₁' = spec.not S₂), from is_false this
+    ) (
+      assume S₂ S₂',
+      have spec.or S₁ S₁' ≠ spec.and S₂ S₂', by contradiction,
+      show decidable (spec.or S₁ S₁' = spec.and S₂ S₂'), from is_false this
+    ) (
+      assume S₂ S₂',
+      have S₁.sizeof < R₁.sizeof, from R₁_id.symm ▸ sizeof_spec_and₁,
+      have decidable (S₁ = S₂), from spec.dec_eq S₁ S₂,
+      have S₁'.sizeof < R₁.sizeof, from R₁_id.symm ▸ sizeof_spec_and₂,
+      have decidable (S₁' = S₂'), from spec.dec_eq S₁' S₂',
+      if h: (S₁ = S₂) ∧ (S₁' = S₂') then (
+        have spec.or S₁ S₁' = spec.or S₂ S₂',
+        from h.left ▸ h.right ▸ rfl,
+        show decidable (spec.or S₁ S₁' = spec.or S₂ S₂'),
+        from is_true this
+      ) else (
+        have spec.or S₁ S₁' ≠ spec.or S₂ S₂', from (
+          assume : spec.or S₁ S₁' = spec.or S₂ S₂',
+          show «false», from h (spec.or.inj this)
+        ),
+        show decidable (spec.or S₁ S₁' = spec.or S₂ S₂'),
+        from is_false this
+      )
+    ) (
+      assume t₂ x₂ S₂ S₂',
+      have spec.or S₁ S₁' ≠ spec.func t₂ x₂ S₂ S₂', by contradiction,
+      show decidable (spec.or S₁ S₁' = spec.func t₂ x₂ S₂ S₂'), from is_false this
+    )
+  ) (
+    assume t₁ x₁ S₁ S₁',
+    assume : z = spec.func t₁ x₁ S₁ S₁',
+    have R₁_id: R₁ = spec.func t₁ x₁ S₁ S₁', from eq.trans h this,
+    show decidable (spec.func t₁ x₁ S₁ S₁' = R₂),
+    from spec.cases_on (λR₂, decidable (spec.func t₁ x₁ S₁ S₁' = R₂)) R₂ (
+      assume t₂,
+      have spec.func t₁ x₁ S₁ S₁' ≠ spec.term t₂, by contradiction,
+      show decidable (spec.func t₁ x₁ S₁ S₁' = spec.term t₂), from is_false this
+    ) (
+      assume S₂,
+      have spec.func t₁ x₁ S₁ S₁' ≠ spec.not S₂, by contradiction,
+      show decidable (spec.func t₁ x₁ S₁ S₁' = spec.not S₂), from is_false this
+    ) (
+      assume S₂ S₂',
+      have spec.func t₁ x₁ S₁ S₁' ≠ spec.and S₂ S₂', by contradiction,
+      show decidable (spec.func t₁ x₁ S₁ S₁' = spec.and S₂ S₂'), from is_false this
+    ) (
+      assume S₂ S₂',
+      have spec.func t₁ x₁ S₁ S₁' ≠ spec.or S₂ S₂', by contradiction,
+      show decidable (spec.func t₁ x₁ S₁ S₁' = spec.or S₂ S₂'), from is_false this
+    ) (
+      assume t₂ x₂ S₂ S₂',
+      have t₁.sizeof < R₁.sizeof, from R₁_id.symm ▸ sizeof_spec_func_t,
+      have decidable (t₁ = t₂), from term.dec_eq t₁ t₂,
+      have S₁.sizeof < R₁.sizeof, from R₁_id.symm ▸ sizeof_spec_func_R,
+      have decidable (S₁ = S₂), from spec.dec_eq S₁ S₂,
+      have S₁'.sizeof < R₁.sizeof, from R₁_id.symm ▸ sizeof_spec_func_S,
+      have decidable (S₁' = S₂'), from spec.dec_eq S₁' S₂',
+      if h: (t₁ = t₂) ∧ (x₁ = x₂) ∧ (S₁ = S₂) ∧ (S₁' = S₂') then (
+        have spec.func t₁ x₁ S₁ S₁' = spec.func t₂ x₂ S₂ S₂',
+        from h.left ▸ h.right.left ▸ h.right.right.left ▸ h.right.right.right ▸ rfl,
+        show decidable (spec.func t₁ x₁ S₁ S₁' = spec.func t₂ x₂ S₂ S₂'),
+        from is_true this
+      ) else (
+        have spec.func t₁ x₁ S₁ S₁' ≠ spec.func t₂ x₂ S₂ S₂', from (
+          assume : spec.func t₁ x₁ S₁ S₁' = spec.func t₂ x₂ S₂ S₂',
+          show «false», from h (spec.func.inj this)
+        ),
+        show decidable (spec.func t₁ x₁ S₁ S₁' = spec.func t₂ x₂ S₂ S₂'),
+        from is_false this
+      )
+    )
+  ) rfl
+
+with env.dec_eq : ∀ (σ₁ σ₂: env), decidable (σ₁ = σ₂)
+| σ₁ σ₂ :=
+  let z := σ₁ in
+  have h: z = σ₁, from rfl,
+  env.cases_on (λσ₁, (z = σ₁) → decidable (σ₁ = σ₂)) σ₁ (
+    assume : z = env.empty,
+    have σ₁_id: σ₁ = env.empty, from eq.trans h this,
+    show decidable (env.empty = σ₂),
+    from env.cases_on (λσ₂, decidable (env.empty = σ₂)) σ₂ (
+      show decidable (env.empty = env.empty), from is_true rfl
+    ) (
+      assume σ₂' x₂ v₂,
+      have env.empty ≠ env.cons σ₂' x₂ v₂, by contradiction,
+      show decidable (env.empty = env.cons σ₂' x₂ v₂), from is_false this
+    )
+  ) (
+    assume σ₁' x₁ v₁,
+    assume : z = env.cons σ₁' x₁ v₁,
+    have σ₁_id: σ₁ = env.cons σ₁' x₁ v₁, from eq.trans h this,
+    show decidable (env.cons σ₁' x₁ v₁ = σ₂),
+    from env.cases_on (λσ₂, decidable (env.cons σ₁' x₁ v₁ = σ₂)) σ₂ (
+      have env.cons σ₁' x₁ v₁ ≠ env.empty, by contradiction,
+      show decidable (env.cons σ₁' x₁ v₁ = env.empty), from is_false this
+    ) (
+      assume σ₂' x₂ v₂,
+      have σ₁'.sizeof < σ₁.sizeof, from σ₁_id.symm ▸ sizeof_env_rest,
+      have decidable (σ₁' = σ₂'), from env.dec_eq σ₁' σ₂',
+      have v₁.sizeof < σ₁.sizeof, from σ₁_id.symm ▸ sizeof_env_value,
+      have decidable (v₁ = v₂), from value.dec_eq v₁ v₂,
+      if h: (σ₁' = σ₂') ∧ (x₁ = x₂) ∧ (v₁ = v₂) then (
+        have env.cons σ₁' x₁ v₁ = env.cons σ₂' x₂ v₂,
+        from h.left ▸ h.right.left ▸ h.right.right ▸ rfl,
+        show decidable (env.cons σ₁' x₁ v₁ = env.cons σ₂' x₂ v₂),
+        from is_true this
+      ) else (
+        have env.cons σ₁' x₁ v₁ ≠ env.cons σ₂' x₂ v₂, from (
+          assume : env.cons σ₁' x₁ v₁ = env.cons σ₂' x₂ v₂,
+          show «false», from h (env.cons.inj this)
+        ),
+        show decidable (env.cons σ₁' x₁ v₁ = env.cons σ₂' x₂ v₂),
+        from is_false this
+      )
+    )
+  ) rfl
+
+with history.dec_eq : ∀ (H₁ H₂: history), decidable (H₁ = H₂)
+| H₁ H₂ :=
+  let z := H₁ in
+  have h: z = H₁, from rfl,
+  history.cases_on (λH₁, (z = H₁) → decidable (H₁ = H₂)) H₁ (
+    assume : z = history.empty,
+    have H₁_id: H₁ = history.empty, from eq.trans h this,
+    show decidable (history.empty = H₂),
+    from history.cases_on (λH₂, decidable (history.empty = H₂)) H₂ (
+      show decidable (history.empty = history.empty), from is_true rfl
+    ) (
+      assume H₂' f₂ x₂ R₂ S₂ e₂ H₂'' σ₂ v₂,
+      have history.empty ≠ history.call H₂' f₂ x₂ R₂ S₂ e₂ H₂'' σ₂ v₂, by contradiction,
+      show decidable (history.empty = history.call H₂' f₂ x₂ R₂ S₂ e₂ H₂'' σ₂ v₂), from is_false this
+    )
+  ) (
+    assume H₁' f₁ x₁ R₁ S₁ e₁ H₁'' σ₁ v₁,
+    assume : z = history.call H₁' f₁ x₁ R₁ S₁ e₁ H₁'' σ₁ v₁,
+    have H₁_id: H₁ = history.call H₁' f₁ x₁ R₁ S₁ e₁ H₁'' σ₁ v₁, from eq.trans h this,
+    show decidable (history.call H₁' f₁ x₁ R₁ S₁ e₁ H₁'' σ₁ v₁ = H₂),
+    from history.cases_on (λH₂, decidable (history.call H₁' f₁ x₁ R₁ S₁ e₁ H₁'' σ₁ v₁ = H₂)) H₂ (
+      have history.call H₁' f₁ x₁ R₁ S₁ e₁ H₁'' σ₁ v₁ ≠ history.empty, by contradiction,
+      show decidable (history.call H₁' f₁ x₁ R₁ S₁ e₁ H₁'' σ₁ v₁ = history.empty), from is_false this
+    ) (
+      assume H₂' f₂ x₂ R₂ S₂ e₂ H₂'' σ₂ v₂,
+      have H₁'.sizeof < H₁.sizeof, from H₁_id.symm ▸ sizeof_history_rest,
+      have decidable (H₁' = H₂'), from history.dec_eq H₁' H₂',
+      have R₁.sizeof < H₁.sizeof, from H₁_id.symm ▸ sizeof_history_R,
+      have decidable (R₁ = R₂), from spec.dec_eq R₁ R₂,
+      have S₁.sizeof < H₁.sizeof, from H₁_id.symm ▸ sizeof_history_S,
+      have decidable (S₁ = S₂), from spec.dec_eq S₁ S₂,
+      have e₁.sizeof < H₁.sizeof, from H₁_id.symm ▸ sizeof_history_e,
+      have decidable (e₁ = e₂), from exp.dec_eq e₁ e₂,
+      have H₁''.sizeof < H₁.sizeof, from H₁_id.symm ▸ sizeof_history_H,
+      have decidable (H₁'' = H₂''), from history.dec_eq H₁'' H₂'',
+      have σ₁.sizeof < H₁.sizeof, from H₁_id.symm ▸ sizeof_history_σ,
+      have decidable (σ₁ = σ₂), from env.dec_eq σ₁ σ₂,
+      have v₁.sizeof < H₁.sizeof, from H₁_id.symm ▸ sizeof_history_v,
+      have decidable (v₁ = v₂), from value.dec_eq v₁ v₂,
+      if h: (H₁' = H₂') ∧ (f₁ = f₂) ∧ (x₁ = x₂) ∧ (R₁ = R₂) ∧ (S₁ = S₂) ∧ 
+            (e₁ = e₂) ∧ (H₁'' = H₂'') ∧ (σ₁ = σ₂) ∧ (v₁ = v₂)
+      then (
+        have history.call H₁' f₁ x₁ R₁ S₁ e₁ H₁'' σ₁ v₁ = history.call H₂' f₂ x₂ R₂ S₂ e₂ H₂'' σ₂ v₂,
+        from h.left ▸ h.right.left ▸ h.right.right.left ▸ h.right.right.right.left ▸
+             h.right.right.right.right.left ▸ h.right.right.right.right.right.left ▸
+             h.right.right.right.right.right.right.left ▸
+             h.right.right.right.right.right.right.right.left ▸
+             h.right.right.right.right.right.right.right.right ▸ rfl,
+        show decidable (history.call H₁' f₁ x₁ R₁ S₁ e₁ H₁'' σ₁ v₁ = history.call H₂' f₂ x₂ R₂ S₂ e₂ H₂'' σ₂ v₂),
+        from is_true this
+      ) else (
+        have history.call H₁' f₁ x₁ R₁ S₁ e₁ H₁'' σ₁ v₁ ≠ history.call H₂' f₂ x₂ R₂ S₂ e₂ H₂'' σ₂ v₂, from (
+          assume : history.call H₁' f₁ x₁ R₁ S₁ e₁ H₁'' σ₁ v₁ = history.call H₂' f₂ x₂ R₂ S₂ e₂ H₂'' σ₂ v₂,
+          show «false», from h (history.call.inj this)
+        ),
+        show decidable (history.call H₁' f₁ x₁ R₁ S₁ e₁ H₁'' σ₁ v₁ = history.call H₂' f₂ x₂ R₂ S₂ e₂ H₂'' σ₂ v₂),
+        from is_false this
+      )
+    )
+  ) rfl
+
+using_well_founded
+{
+  rel_tac := λ _ _, `[exact wf_measure],
+  dec_tac := tactic.assumption
+}
+
+instance : decidable_eq value := value.dec_eq
